@prefix fibo.FBC.DebtAndEquities.CreditEvents: <https://spec.edmcouncil.org/fibo/ontology/FBC/DebtAndEquities/CreditEvents/> .

@prefix rdf: <http://www.w3.org/1999/02/22-rdf-syntax-ns#>.
@prefix rdfs: <http://www.w3.org/2000/01/rdf-schema#>.
@prefix xsd: <http://www.w3.org/2001/XMLSchema#>.
@prefix xml: <http://www.w3.org/XML/1998/namespace>.
@prefix cmns-av: <https://www.omg.org/spec/Commons/AnnotationVocabulary/>.
@prefix cmns-cxtdsg: <https://www.omg.org/spec/Commons/ContextualDesignators/>.
@prefix cmns-dt: <https://www.omg.org/spec/Commons/DatesAndTimes/>.
@prefix cmns-org: <https://www.omg.org/spec/Commons/Organizations/>.
@prefix dcterms: <http://purl.org/dc/terms/>.
@prefix fibo-fbc-dae-cre: <https://spec.edmcouncil.org/fibo/ontology/FBC/DebtAndEquities/CreditEvents/>.
@prefix fibo-fbc-dae-dbt: <https://spec.edmcouncil.org/fibo/ontology/FBC/DebtAndEquities/Debt/>.
@prefix fibo-fnd-acc-cur: <https://spec.edmcouncil.org/fibo/ontology/FND/Accounting/CurrencyAmount/>.
@prefix fibo-fnd-agr-ctr: <https://spec.edmcouncil.org/fibo/ontology/FND/Agreements/Contracts/>.
@prefix fibo-fnd-dt-oc: <https://spec.edmcouncil.org/fibo/ontology/FND/DatesAndTimes/Occurrences/>.
@prefix fibo-fnd-law-lcap: <https://spec.edmcouncil.org/fibo/ontology/FND/Law/LegalCapacity/>.
@prefix fibo-fnd-pas-psch: <https://spec.edmcouncil.org/fibo/ontology/FND/ProductsAndServices/PaymentsAndSchedules/>.
@prefix fibo-fnd-rel-rel: <https://spec.edmcouncil.org/fibo/ontology/FND/Relations/Relations/>.
@prefix fibo-fnd-utl-av: <https://spec.edmcouncil.org/fibo/ontology/FND/Utilities/AnnotationVocabulary/>.
@prefix owl: <http://www.w3.org/2002/07/owl#>.
@prefix skos: <http://www.w3.org/2004/02/skos/core#>.

_:autos1095 rdf:first fibo-fbc-dae-dbt:CreditAgreement;
            rdf:rest _:autos1096.
_:autos1096 rdf:first fibo-fnd-pas-psch:PaymentObligation;
            rdf:rest rdf:nil.
fibo-fbc-dae-cre: dcterms:abstract """This ontology defines a range of credit events, that is events in which some payment or payments are not made. These include credit events relating to a specific debt obligation and events relating to the business entity as a whole. 
		Note: the events defined herein are primarily business rather than consumer oriented, and are specified fairly generally. Many credit events are jurisdiction-specific, such as Chapter 11 restructuring and Chapter 7 bankruptcy in the United States. This ontology is designed to facilitate jurisdiction and instrument-specific extensions as needed.""";
                  dcterms:license """Copyright (c) 2013-2025 EDM Council, Inc.
Copyright (c) 2013-2025 Object Management Group, Inc.
		
Permission is hereby granted, free of charge, to any person obtaining a copy of this software and associated documentation files (the 'Software'), to deal in the Software without restriction, including without limitation the rights to use, copy, modify, merge, publish, distribute, sublicense, and/or sell copies of the Software, and to permit persons to whom the Software is furnished to do so, subject to the following conditions:

The above copyright notice and this permission notice shall be included in all copies or substantial portions of the Software.

THE SOFTWARE IS PROVIDED 'AS IS', WITHOUT WARRANTY OF ANY KIND, EXPRESS OR IMPLIED, INCLUDING BUT NOT LIMITED TO THE WARRANTIES OF MERCHANTABILITY, FITNESS FOR A PARTICULAR PURPOSE AND NONINFRINGEMENT. IN NO EVENT SHALL THE AUTHORS OR COPYRIGHT HOLDERS BE LIABLE FOR ANY CLAIM, DAMAGES OR OTHER LIABILITY, WHETHER IN AN ACTION OF CONTRACT, TORT OR OTHERWISE, ARISING FROM, OUT OF OR IN CONNECTION WITH THE SOFTWARE OR THE USE OR OTHER DEALINGS IN THE SOFTWARE.
		
		See https://opensource.org/licenses/MIT.""";
                  a owl:Ontology;
                  rdfs:label "Credit Events Ontology"@en;
                  owl:imports <https://spec.edmcouncil.org/fibo/ontology/master/latest/FBC/DebtAndEquities/Debt/>,
                              <https://spec.edmcouncil.org/fibo/ontology/master/latest/FND/Accounting/CurrencyAmount/>,
                              <https://spec.edmcouncil.org/fibo/ontology/master/latest/FND/Agreements/Contracts/>,
                              <https://spec.edmcouncil.org/fibo/ontology/master/latest/FND/DatesAndTimes/Occurrences/>,
                              <https://spec.edmcouncil.org/fibo/ontology/master/latest/FND/Law/LegalCapacity/>,
                              <https://spec.edmcouncil.org/fibo/ontology/master/latest/FND/ProductsAndServices/PaymentsAndSchedules/>,
                              <https://spec.edmcouncil.org/fibo/ontology/master/latest/FND/Relations/Relations/>,
                              <https://spec.edmcouncil.org/fibo/ontology/master/latest/FND/Utilities/AnnotationVocabulary/>,
                              cmns-av:,
                              cmns-cxtdsg:,
                              cmns-dt:,
                              cmns-org:;
                  owl:versionIRI <https://spec.edmcouncil.org/fibo/ontology/master/latest/FBC/DebtAndEquities/CreditEvents/>;
                  skos:changeNote "The https://spec.edmcouncil.org/fibo/ontology/FBC/DebtAndEquities/CreditEvents.rdf version of the ontology was modified to replace additional content that is now available in the OMG Commons Ontology Library (Commons) v1.2 (FND-389).",
                                  "The https://spec.edmcouncil.org/fibo/ontology/FBC/DebtAndEquities/CreditEvents.rdf version of the ontology was modified to use the Commons Ontology Library (Commons) Annotation Vocabulary rather than the OMG's Specification Metadata vocabulary.",
                                  "The https://spec.edmcouncil.org/fibo/ontology/FBC/DebtAndEquities/CreditEvents.rdf version of this ontology was modified to add the currency pertinent to a credit agreement (DER-55).",
                                  "The https://spec.edmcouncil.org/fibo/ontology/FBC/DebtAndEquities/CreditEvents.rdf version of this ontology was modified to move the property, 'is conferred on' to the Legal Capacity ontology and to use the Commons Ontology Library (Commons) rather than the OMG's Languages, Countries and Codes (LCC), eliminating redundancies in FIBO as appropriate.",
                                  "The https://spec.edmcouncil.org/fibo/ontology/FBC/DebtAndEquities/CreditEvents.rdf version of this ontology was modified to replace content that is now available in the OMG Commons Ontology Library (Commons) v1.1 (FND-380).",
                                  "The https://spec.edmcouncil.org/fibo/ontology/FBC/DebtAndEquities/CreditEvents.rdf version of this ontology was revised to address text formatting issues uncovered by hygiene testing.",
                                  "The https://spec.edmcouncil.org/fibo/ontology/FBC/DebtAndEquities/CreditEvents.rdf version of this ontology was revised to augment the definition of obligation-specific event with an optional default threshold to better support credit default swaps.",
                                  "The https://spec.edmcouncil.org/fibo/ontology/FBC/DebtAndEquities/CreditEvents.rdf version of this ontology was revised to move a restriction involving breach of covenant from credit event, since not all credit events involve breaches, to default event, and loosen the constraint since a breach depends on the contract.";
                  fibo-fnd-utl-av:hasMaturityLevel fibo-fnd-utl-av:Release;
                  cmns-av:copyright "Copyright (c) 2018-2025 EDM Council, Inc.",
                                    "Copyright (c) 2020-2025 Object Management Group, Inc.".
fibo-fbc-dae-cre:Bankruptcy a owl:Class;
                            rdfs:isDefinedBy fibo-fbc-dae-cre:;
                            rdfs:label "bankruptcy"@en;
                            rdfs:subClassOf fibo-fbc-dae-cre:EntitySpecificCreditEvent;
                            skos:definition "credit event involving a change in state or condition in which a party becomes insolvent"@en;
                            cmns-av:adaptedFrom "Barron's Dictionary of Banking Terms, Sixth Edition, 2012",
                                                "https://thelawdictionary.org/bankruptcy/"^^xsd:anyURI.
fibo-fbc-dae-cre:CreditEvent a owl:Class;
                             rdfs:isDefinedBy fibo-fbc-dae-cre:;
                             rdfs:label "credit event"@en;
                             rdfs:subClassOf fibo-fnd-dt-oc:Occurrence;
                             skos:definition "event signifying a sudden change in credit standing, such as bankruptcy or a violation of a bond indenture or loan agreement, that raises doubts about the party's ability to meet current or future obligations"@en.
fibo-fbc-dae-cre:CrossDefaultProvision a owl:Class;
                                       rdfs:isDefinedBy fibo-fbc-dae-cre:;
                                       rdfs:label "cross default provision"@en;
                                       rdfs:subClassOf fibo-fnd-agr-ctr:ConditionPrecedent,
                                                       [a owl:Restriction ; 
                                                        owl:onProperty fibo-fbc-dae-cre:hasDefaultThresholdAmount ; 
                                                        owl:onClass fibo-fnd-acc-cur:MonetaryAmount ; 
                                                        owl:minQualifiedCardinality "0"^^xsd:nonNegativeInteger],
                                                       [a owl:Restriction ; 
                                                        owl:onProperty cmns-cxtdsg:appliesTo ; 
                                                        owl:someValuesFrom fibo-fbc-dae-dbt:CreditAgreement];
                                       skos:definition "contract provision that triggers a default under one contract if the borrower defaults on another related obligation";
                                       cmns-av:explanatoryNote "Cross default provisions are commonly found in loans, bond indentures, syndicated loans, and other instruments such as certain master agreements (e.g., derivatives transactions master agreements).".
fibo-fbc-dae-cre:DefaultEvent a owl:Class;
                              rdfs:isDefinedBy fibo-fbc-dae-cre:;
                              rdfs:label "default event"@en;
                              rdfs:subClassOf fibo-fbc-dae-cre:ObligationSpecificCreditEvent,
                                              [a owl:Restriction ; 
                                               owl:onProperty fibo-fnd-rel-rel:exemplifies ; 
                                               owl:onClass fibo-fnd-agr-ctr:BreachOfCovenant ; 
                                               owl:minQualifiedCardinality "0"^^xsd:nonNegativeInteger];
                              skos:definition "credit event representing a failure to meet a contractual obligation, such as failure to repay a debt including interest or principal on a loan or security"@en;
                              cmns-av:explanatoryNote "A default can occur when a borrower is unable to make timely payments, misses payments, or avoids or stops making payments, typically with respect to a single transaction. A default has adverse effects on the borrower's credit and ability to borrow in the future, and allows the creditor to demand immediate repayment of the obligation in full."@en.
fibo-fbc-dae-cre:DistressedRatingsDowngrade a owl:Class;
                                            rdfs:isDefinedBy fibo-fbc-dae-cre:;
                                            rdfs:label "distressed ratings downgrade"@en;
                                            rdfs:subClassOf fibo-fbc-dae-cre:Downgrade;
                                            skos:definition "credit event triggered when the credit rating of an obligation is downgraded to a distressed debt level"@en.
fibo-fbc-dae-cre:Downgrade a owl:Class;
                           rdfs:isDefinedBy fibo-fbc-dae-cre:;
                           rdfs:label "downgrade"@en;
                           rdfs:subClassOf fibo-fbc-dae-cre:CreditEvent;
                           skos:definition "credit event triggered when the credit rating of a party or obligation is lowered"@en;
                           skos:example "On October 17, 2013, Dagong Global Credit Rating downgraded the United States from A to A- and maintained a negative outlook on the country's credit."@en.
fibo-fbc-dae-cre:EntitySpecificCreditEvent a owl:Class;
                                           rdfs:isDefinedBy fibo-fbc-dae-cre:;
                                           rdfs:label "entity-specific credit event"@en;
                                           rdfs:subClassOf fibo-fbc-dae-cre:CreditEvent,
                                                           [a owl:Restriction ; 
                                                            owl:onProperty cmns-cxtdsg:appliesTo ; 
                                                            owl:someValuesFrom cmns-org:LegalPerson];
                                           skos:definition "credit event that applies to a given legal person"@en.
fibo-fbc-dae-cre:FailureToPay a owl:Class;
                              rdfs:isDefinedBy fibo-fbc-dae-cre:;
                              rdfs:label "failure to pay"@en;
                              rdfs:subClassOf fibo-fbc-dae-cre:DefaultEvent,
                                              [a owl:Restriction ; 
                                               owl:onProperty fibo-fbc-dae-cre:hasGracePeriod ; 
                                               owl:onClass cmns-dt:DatePeriod ; 
                                               owl:maxQualifiedCardinality "1"^^xsd:nonNegativeInteger];
                              skos:definition "default event that is triggered following any applicable grace period in which a payment obligation is missed"@en.
fibo-fbc-dae-cre:FailureToPayInterest a owl:Class;
                                      rdfs:isDefinedBy fibo-fbc-dae-cre:;
                                      rdfs:label "failure to pay interest"@en;
                                      rdfs:subClassOf fibo-fbc-dae-cre:FailureToPay;
                                      skos:definition "default event that where either an expected interest payment is missed altogether or the amount paid is less than the required amount"@en.
fibo-fbc-dae-cre:FailureToPayPrincipal a owl:Class;
                                       rdfs:isDefinedBy fibo-fbc-dae-cre:;
                                       rdfs:label "failure to pay principal"@en;
                                       rdfs:subClassOf fibo-fbc-dae-cre:FailureToPay;
                                       skos:definition "default event that where either an expected principal payment is missed altogether or the amount paid is less than the required amount"@en.
fibo-fbc-dae-cre:FilingForBankruptcy a owl:Class;
                                     rdfs:isDefinedBy fibo-fbc-dae-cre:;
                                     rdfs:label "filing for bankruptcy"@en;
                                     rdfs:subClassOf fibo-fbc-dae-cre:EntitySpecificCreditEvent;
                                     skos:definition "credit event that involves a request to a court to be recognized as bankrupt"@en;
                                     cmns-av:explanatoryNote "The bankruptcy process is initiated via a petition filed by the debtor or on behalf of creditors. The debtor's assets may be used to repay a portion of outstanding debt as specified by the court or a court-appointed individual."@en.
fibo-fbc-dae-cre:HardCreditEvent a owl:Class;
                                 rdfs:isDefinedBy fibo-fbc-dae-cre:;
                                 rdfs:label "hard credit event"@en;
                                 rdfs:subClassOf fibo-fbc-dae-cre:DefaultEvent;
                                 skos:definition "default event that is not repairable"@en.
fibo-fbc-dae-cre:InstallmentDefault a owl:Class;
                                    rdfs:isDefinedBy fibo-fbc-dae-cre:;
                                    rdfs:label "installment default"@en;
                                    rdfs:subClassOf fibo-fbc-dae-cre:DefaultEvent;
                                    skos:definition "default event involving non-payment of several installment payments as scheduled in the terms of the agreement, or non-payment of a call by the beneficial owner"@en;
                                    cmns-av:explanatoryNote "The latter may result in a court action by the issuer or the sale of the securities to recover costs and/or a forfeit of partially paid securities."@en.
fibo-fbc-dae-cre:InterestObligationInLightOfDefault a owl:Class;
                                                    rdfs:isDefinedBy fibo-fbc-dae-cre:;
                                                    rdfs:label "interest obligation in light of default"@en;
                                                    rdfs:subClassOf fibo-fnd-law-lcap:ContingentObligation,
                                                                    fibo-fnd-law-lcap:ContractualObligation,
                                                                    [a owl:Restriction ; 
                                                                     owl:onProperty fibo-fbc-dae-cre:hasDefaultInterestCompoundingBasis ; 
                                                                     owl:onClass cmns-dt:DatePeriod ; 
                                                                     owl:maxQualifiedCardinality "1"^^xsd:nonNegativeInteger],
                                                                    [a owl:Restriction ; 
                                                                     owl:onProperty fibo-fbc-dae-cre:isDefaultInterestApplicable ; 
                                                                     owl:maxQualifiedCardinality "1"^^xsd:nonNegativeInteger ; 
                                                                     owl:onDataRange xsd:boolean],
                                                                    [a owl:Restriction ; 
                                                                     owl:onProperty fibo-fnd-rel-rel:isMandatedBy ; 
                                                                     owl:someValuesFrom fibo-fnd-pas-psch:PaymentObligation ; 
                                                                     owl:someValuesFrom [a owl:Class ; 
                                                                                         owl:unionOf _:autos1095]];
                                                    skos:definition "obligation in respect of default(s) in the performance of any payment obligation"@en;
                                                    skos:example "Prior to the occurrence or effective designation of an early termination date in respect of the relevant transaction, a party that defaults in the performance of any payment obligation will, to the extent permitted by law (and in the case of an ISDA Master Agreement is subject to Section 6(c)), be required to pay interest (before as well as after judgment) on the overdue amount to the other party on demand in the same currency as such overdue amount, for the period from (and including) the original due date for payment to (but excluding) the date of actual payment, at the default rate. Such interest will be calculated on the basis of daily compounding and the actual number of days elapsed."@en.
fibo-fbc-dae-cre:MaturityExtension a owl:Class;
                                   rdfs:isDefinedBy fibo-fbc-dae-cre:;
                                   rdfs:label "maturity extension"@en;
                                   rdfs:subClassOf fibo-fbc-dae-cre:ObligationSpecificCreditEvent;
                                   skos:definition "credit event involving extension of payments beyond the original maturity date of the obligation"@en;
                                   cmns-av:explanatoryNote "As stipulated in the terms and conditions for a bond, for example, the issuer or the bondholder may prolong the maturity date. After extension, the security may differ from original issue (new rate or maturity date). May be subject to bondholder's approval."@en.
fibo-fbc-dae-cre:Moratorium a owl:Class;
                            rdfs:isDefinedBy fibo-fbc-dae-cre:;
                            rdfs:label "moratorium"@en;
                            rdfs:subClassOf fibo-fbc-dae-cre:EntitySpecificCreditEvent;
                            skos:definition "entity-specific credit event involving a temporary suspension of payments until related issues are resolved"@en;
                            cmns-av:explanatoryNote "A moratorium may be a legally-mandated hiatus in debt collection as a part of a bankruptcy process."@en.
fibo-fbc-dae-cre:ObligationAcceleration a owl:Class;
                                        rdfs:isDefinedBy fibo-fbc-dae-cre:;
                                        rdfs:label "obligation acceleration"@en;
                                        rdfs:subClassOf fibo-fbc-dae-cre:ObligationSpecificCreditEvent;
                                        skos:definition "credit event triggered when one or more reference obligations become immediately due and payable as a result of a default or covenant breach on the reference entity's other debt instruments, subject to a materiality threshold"@en.
fibo-fbc-dae-cre:ObligationDefault a owl:Class;
                                   rdfs:isDefinedBy fibo-fbc-dae-cre:;
                                   rdfs:label "obligation default"@en;
                                   rdfs:subClassOf fibo-fbc-dae-cre:DefaultEvent,
                                                   fibo-fbc-dae-cre:ObligationSpecificCreditEvent;
                                   skos:definition "credit event triggered as a result of an obligation-specific default"@en.
fibo-fbc-dae-cre:ObligationRestructuring a owl:Class;
                                         rdfs:isDefinedBy fibo-fbc-dae-cre:;
                                         rdfs:label "obligation restructuring"@en;
                                         rdfs:subClassOf fibo-fbc-dae-cre:ObligationSpecificCreditEvent;
                                         skos:definition "credit event that materially impacts an obligation, such as an interest rate reduction, principal reduction, deferral of interest or principal, change in priority ranking, or change in currency or composition of payment"@en.
fibo-fbc-dae-cre:ObligationSpecificCreditEvent a owl:Class;
                                               rdfs:isDefinedBy fibo-fbc-dae-cre:;
                                               rdfs:label "obligation-specific credit event"@en;
                                               rdfs:subClassOf fibo-fbc-dae-cre:CreditEvent,
                                                               [a owl:Restriction ; 
                                                                owl:onProperty fibo-fbc-dae-cre:hasDefaultThresholdAmount ; 
                                                                owl:onClass fibo-fnd-acc-cur:MonetaryAmount ; 
                                                                owl:minQualifiedCardinality "0"^^xsd:nonNegativeInteger],
                                                               [a owl:Restriction ; 
                                                                owl:onProperty cmns-cxtdsg:appliesTo ; 
                                                                owl:someValuesFrom fibo-fbc-dae-dbt:CreditAgreement];
                                               skos:definition "credit event that relates to an individual credit agreement or debt instrument (reference obligation)"@en.
fibo-fbc-dae-cre:Repudiation a owl:Class;
                             rdfs:isDefinedBy fibo-fbc-dae-cre:;
                             rdfs:label "repudiation"@en;
                             rdfs:subClassOf fibo-fbc-dae-cre:ObligationSpecificCreditEvent;
                             skos:definition "credit event involving the refusal to honor the terms of a contract"@en.
fibo-fbc-dae-cre:SoftCreditEvent a owl:Class;
                                 rdfs:isDefinedBy fibo-fbc-dae-cre:;
                                 rdfs:label "soft credit event"@en;
                                 rdfs:subClassOf fibo-fbc-dae-cre:DefaultEvent;
                                 owl:disjointWith fibo-fbc-dae-cre:HardCreditEvent;
                                 skos:definition "default event that is repairable"@en;
                                 cmns-av:explanatoryNote "If the default is not repaired within a grace period, then a failure to repair (failure to pay) credit event is triggered, potentially as a hard default."@en.
fibo-fbc-dae-cre:WriteDown a owl:Class;
                           rdfs:isDefinedBy fibo-fbc-dae-cre:;
                           rdfs:label "write-down"@en;
                           rdfs:subClassOf fibo-fbc-dae-cre:ObligationSpecificCreditEvent;
                           skos:definition "obligation-specific credit event whereby the book value of the obligation, such as the outstanding principal amount, is reduced"@en.
fibo-fbc-dae-cre:hasDefaultInterestCompoundingBasis a owl:ObjectProperty;
                                                    rdfs:domain fibo-fbc-dae-cre:InterestObligationInLightOfDefault;
                                                    rdfs:isDefinedBy fibo-fbc-dae-cre:;
                                                    rdfs:label "has default interest compounding basis"@en;
                                                    rdfs:range cmns-dt:DatePeriod;
                                                    rdfs:subPropertyOf cmns-dt:hasDatePeriod;
                                                    skos:definition "indicates the basis on which default interest is to be calculated, as a period of time"@en.
fibo-fbc-dae-cre:hasDefaultThresholdAmount a owl:ObjectProperty;
                                           rdfs:isDefinedBy fibo-fbc-dae-cre:;
                                           rdfs:label "has default threshold amount"@en;
                                           rdfs:range fibo-fnd-acc-cur:MonetaryAmount;
                                           rdfs:subPropertyOf fibo-fnd-acc-cur:hasMonetaryAmount;
                                           skos:definition "specifies an amount of money that triggers a failure to pay, repudiation/moratorium or restructuring event"@en.
fibo-fbc-dae-cre:hasGracePeriod a owl:ObjectProperty;
                                rdfs:isDefinedBy fibo-fbc-dae-cre:;
                                rdfs:label "has grace period"@en;
                                rdfs:range cmns-dt:DatePeriod;
                                rdfs:subPropertyOf cmns-dt:hasDatePeriod;
                                skos:definition "window following any payment due date during which a party must fulfill its obligations before a failure to pay credit event occurs"@en;
                                cmns-av:explanatoryNote "Note that this may be a period denominated in business days or calendar days."@en.
fibo-fbc-dae-cre:involvesMultipleEvents a owl:DatatypeProperty;
                                        rdfs:domain fibo-fbc-dae-cre:ObligationRestructuring;
                                        rdfs:isDefinedBy fibo-fbc-dae-cre:;
                                        rdfs:label "involves multiple events"@en;
                                        rdfs:range xsd:boolean;
                                        skos:definition "indicates that the restructuring spans more than one credit event"@en.
fibo-fbc-dae-cre:isDefaultInterestApplicable a owl:DatatypeProperty;
                                             rdfs:domain fibo-fbc-dae-cre:InterestObligationInLightOfDefault;
                                             rdfs:isDefinedBy fibo-fbc-dae-cre:;
                                             rdfs:label "is default interest applicable"@en;
                                             rdfs:range xsd:boolean;
                                             skos:definition "indicates whether a party that defaults in the performance of any payment obligation is, to the extent permitted by law and the applicable agreement, required to pay interest (before as well as after judgment) on the overdue amount to the other party on demand in the same currency as such overdue amount, for the period from (and including) the original due date for payment to (but excluding) the date of actual payment"@en.
fibo-fbc-dae-cre:isGracePeriodExtendable a owl:DatatypeProperty;
                                         rdfs:isDefinedBy fibo-fbc-dae-cre:;
                                         rdfs:label "is grace period extendable"@en;
                                         rdfs:range xsd:boolean;
                                         skos:definition "indicates whether or not the grace period may be extended, which may be jurisdiction specific"@en.
