@prefix fibo.SEC.Funds.CollectiveInvestmentVehicles: <https://spec.edmcouncil.org/fibo/ontology/SEC/Funds/CollectiveInvestmentVehicles/> .

@prefix rdf: <http://www.w3.org/1999/02/22-rdf-syntax-ns#>.
@prefix rdfs: <http://www.w3.org/2000/01/rdf-schema#>.
@prefix xsd: <http://www.w3.org/2001/XMLSchema#>.
@prefix xml: <http://www.w3.org/XML/1998/namespace>.
@prefix cmns-av: <https://www.omg.org/spec/Commons/AnnotationVocabulary/>.
@prefix cmns-cls: <https://www.omg.org/spec/Commons/Classifiers/>.
@prefix cmns-col: <https://www.omg.org/spec/Commons/Collections/>.
@prefix cmns-cxtdsg: <https://www.omg.org/spec/Commons/ContextualDesignators/>.
@prefix cmns-doc: <https://www.omg.org/spec/Commons/Documents/>.
@prefix cmns-dsg: <https://www.omg.org/spec/Commons/Designators/>.
@prefix cmns-dt: <https://www.omg.org/spec/Commons/DatesAndTimes/>.
@prefix cmns-loc: <https://www.omg.org/spec/Commons/Locations/>.
@prefix cmns-org: <https://www.omg.org/spec/Commons/Organizations/>.
@prefix cmns-pts: <https://www.omg.org/spec/Commons/PartiesAndSituations/>.
@prefix cmns-qtu: <https://www.omg.org/spec/Commons/QuantitiesAndUnits/>.
@prefix cmns-rga: <https://www.omg.org/spec/Commons/RegulatoryAgencies/>.
@prefix cmns-rlcmp: <https://www.omg.org/spec/Commons/RolesAndCompositions/>.
@prefix dcterms: <http://purl.org/dc/terms/>.
@prefix fibo-be-fct-pub: <https://spec.edmcouncil.org/fibo/ontology/BE/FunctionalEntities/Publishers/>.
@prefix fibo-be-ge-euj: <https://spec.edmcouncil.org/fibo/ontology/BE/GovernmentEntities/EuropeanJurisdiction/EUGovernmentEntitiesAndJurisdictions/>.
@prefix fibo-be-le-cb: <https://spec.edmcouncil.org/fibo/ontology/BE/LegalEntities/CorporateBodies/>.
@prefix fibo-be-oac-cown: <https://spec.edmcouncil.org/fibo/ontology/BE/OwnershipAndControl/CorporateOwnership/>.
@prefix fibo-be-oac-exec: <https://spec.edmcouncil.org/fibo/ontology/BE/OwnershipAndControl/Executives/>.
@prefix fibo-be-oac-opty: <https://spec.edmcouncil.org/fibo/ontology/BE/OwnershipAndControl/OwnershipParties/>.
@prefix fibo-fbc-fct-fse: <https://spec.edmcouncil.org/fibo/ontology/FBC/FunctionalEntities/FinancialServicesEntities/>.
@prefix fibo-fbc-fi-fi: <https://spec.edmcouncil.org/fibo/ontology/FBC/FinancialInstruments/FinancialInstruments/>.
@prefix fibo-fbc-fi-stl: <https://spec.edmcouncil.org/fibo/ontology/FBC/FinancialInstruments/Settlement/>.
@prefix fibo-fbc-pas-caa: <https://spec.edmcouncil.org/fibo/ontology/FBC/ProductsAndServices/ClientsAndAccounts/>.
@prefix fibo-fbc-pas-fpas: <https://spec.edmcouncil.org/fibo/ontology/FBC/ProductsAndServices/FinancialProductsAndServices/>.
@prefix fibo-fnd-acc-cur: <https://spec.edmcouncil.org/fibo/ontology/FND/Accounting/CurrencyAmount/>.
@prefix fibo-fnd-agr-ctr: <https://spec.edmcouncil.org/fibo/ontology/FND/Agreements/Contracts/>.
@prefix fibo-fnd-arr-lif: <https://spec.edmcouncil.org/fibo/ontology/FND/Arrangements/Lifecycles/>.
@prefix fibo-fnd-arr-rt: <https://spec.edmcouncil.org/fibo/ontology/FND/Arrangements/Ratings/>.
@prefix fibo-fnd-dt-bd: <https://spec.edmcouncil.org/fibo/ontology/FND/DatesAndTimes/BusinessDates/>.
@prefix fibo-fnd-dt-fd: <https://spec.edmcouncil.org/fibo/ontology/FND/DatesAndTimes/FinancialDates/>.
@prefix fibo-fnd-gao-obj: <https://spec.edmcouncil.org/fibo/ontology/FND/GoalsAndObjectives/Objectives/>.
@prefix fibo-fnd-law-cor: <https://spec.edmcouncil.org/fibo/ontology/FND/Law/LegalCore/>.
@prefix fibo-fnd-law-lcap: <https://spec.edmcouncil.org/fibo/ontology/FND/Law/LegalCapacity/>.
@prefix fibo-fnd-plc-rp: <https://spec.edmcouncil.org/fibo/ontology/FND/Places/RealProperty/>.
@prefix fibo-fnd-rel-rel: <https://spec.edmcouncil.org/fibo/ontology/FND/Relations/Relations/>.
@prefix fibo-fnd-utl-av: <https://spec.edmcouncil.org/fibo/ontology/FND/Utilities/AnnotationVocabulary/>.
@prefix fibo-ind-ind-ind: <https://spec.edmcouncil.org/fibo/ontology/IND/Indicators/Indicators/>.
@prefix fibo-sec-eq-eq: <https://spec.edmcouncil.org/fibo/ontology/SEC/Equities/EquityInstruments/>.
@prefix fibo-sec-fund-civ: <https://spec.edmcouncil.org/fibo/ontology/SEC/Funds/CollectiveInvestmentVehicles/>.
@prefix fibo-sec-fund-fund: <https://spec.edmcouncil.org/fibo/ontology/SEC/Funds/Funds/>.
@prefix fibo-sec-sec-ast: <https://spec.edmcouncil.org/fibo/ontology/SEC/Securities/SecurityAssets/>.
@prefix fibo-sec-sec-cls: <https://spec.edmcouncil.org/fibo/ontology/SEC/Securities/SecuritiesClassification/>.
@prefix fibo-sec-sec-iss: <https://spec.edmcouncil.org/fibo/ontology/SEC/Securities/SecuritiesIssuance/>.
@prefix fibo-sec-sec-pls: <https://spec.edmcouncil.org/fibo/ontology/SEC/Securities/Pools/>.
@prefix fibo-sec-sec-rst: <https://spec.edmcouncil.org/fibo/ontology/SEC/Securities/SecuritiesRestrictions/>.
@prefix owl: <http://www.w3.org/2002/07/owl#>.
@prefix skos: <http://www.w3.org/2004/02/skos/core#>.

fibo-sec-fund-civ: dcterms:abstract "Reference data terms and non time dependent facts about funds and CIVs.";
                   dcterms:license """Copyright (c) 2013-2025 EDM Council, Inc.
Copyright (c) 2013-2025 Object Management Group, Inc.

Permission is hereby granted, free of charge, to any person obtaining a copy of this software and associated documentation files (the 'Software'), to deal in the Software without restriction, including without limitation the rights to use, copy, modify, merge, publish, distribute, sublicense, and/or sell copies of the Software, and to permit persons to whom the Software is furnished to do so, subject to the following conditions:

The above copyright notice and this permission notice shall be included in all copies or substantial portions of the Software.

THE SOFTWARE IS PROVIDED 'AS IS', WITHOUT WARRANTY OF ANY KIND, EXPRESS OR IMPLIED, INCLUDING BUT NOT LIMITED TO THE WARRANTIES OF MERCHANTABILITY, FITNESS FOR A PARTICULAR PURPOSE AND NONINFRINGEMENT. IN NO EVENT SHALL THE AUTHORS OR COPYRIGHT HOLDERS BE LIABLE FOR ANY CLAIM, DAMAGES OR OTHER LIABILITY, WHETHER IN AN ACTION OF CONTRACT, TORT OR OTHERWISE, ARISING FROM, OUT OF OR IN CONNECTION WITH THE SOFTWARE OR THE USE OR OTHER DEALINGS IN THE SOFTWARE.
		
		See https://opensource.org/licenses/MIT.""";
                   a owl:Ontology;
                   rdfs:label "Collective Investment Vehicles Ontology"@en;
                   owl:imports <https://spec.edmcouncil.org/fibo/ontology/master/latest/BE/FunctionalEntities/Publishers/>,
                               <https://spec.edmcouncil.org/fibo/ontology/master/latest/BE/GovernmentEntities/EuropeanJurisdiction/EUGovernmentEntitiesAndJurisdictions/>,
                               <https://spec.edmcouncil.org/fibo/ontology/master/latest/BE/LegalEntities/CorporateBodies/>,
                               <https://spec.edmcouncil.org/fibo/ontology/master/latest/BE/LegalEntities/FormalBusinessOrganizations/>,
                               <https://spec.edmcouncil.org/fibo/ontology/master/latest/BE/LegalEntities/LegalPersons/>,
                               <https://spec.edmcouncil.org/fibo/ontology/master/latest/BE/OwnershipAndControl/CorporateOwnership/>,
                               <https://spec.edmcouncil.org/fibo/ontology/master/latest/BE/OwnershipAndControl/Executives/>,
                               <https://spec.edmcouncil.org/fibo/ontology/master/latest/BE/OwnershipAndControl/OwnershipParties/>,
                               <https://spec.edmcouncil.org/fibo/ontology/master/latest/FBC/DebtAndEquities/Debt/>,
                               <https://spec.edmcouncil.org/fibo/ontology/master/latest/FBC/FinancialInstruments/FinancialInstruments/>,
                               <https://spec.edmcouncil.org/fibo/ontology/master/latest/FBC/FinancialInstruments/Settlement/>,
                               <https://spec.edmcouncil.org/fibo/ontology/master/latest/FBC/FunctionalEntities/FinancialServicesEntities/>,
                               <https://spec.edmcouncil.org/fibo/ontology/master/latest/FBC/ProductsAndServices/ClientsAndAccounts/>,
                               <https://spec.edmcouncil.org/fibo/ontology/master/latest/FBC/ProductsAndServices/FinancialProductsAndServices/>,
                               <https://spec.edmcouncil.org/fibo/ontology/master/latest/FND/Accounting/AccountingEquity/>,
                               <https://spec.edmcouncil.org/fibo/ontology/master/latest/FND/Accounting/CurrencyAmount/>,
                               <https://spec.edmcouncil.org/fibo/ontology/master/latest/FND/Agreements/Contracts/>,
                               <https://spec.edmcouncil.org/fibo/ontology/master/latest/FND/Arrangements/Lifecycles/>,
                               <https://spec.edmcouncil.org/fibo/ontology/master/latest/FND/Arrangements/Ratings/>,
                               <https://spec.edmcouncil.org/fibo/ontology/master/latest/FND/DatesAndTimes/BusinessDates/>,
                               <https://spec.edmcouncil.org/fibo/ontology/master/latest/FND/DatesAndTimes/FinancialDates/>,
                               <https://spec.edmcouncil.org/fibo/ontology/master/latest/FND/GoalsAndObjectives/Objectives/>,
                               <https://spec.edmcouncil.org/fibo/ontology/master/latest/FND/Law/LegalCapacity/>,
                               <https://spec.edmcouncil.org/fibo/ontology/master/latest/FND/Law/LegalCore/>,
                               <https://spec.edmcouncil.org/fibo/ontology/master/latest/FND/OwnershipAndControl/Ownership/>,
                               <https://spec.edmcouncil.org/fibo/ontology/master/latest/FND/Places/RealProperty/>,
                               <https://spec.edmcouncil.org/fibo/ontology/master/latest/FND/Relations/Relations/>,
                               <https://spec.edmcouncil.org/fibo/ontology/master/latest/FND/Utilities/AnnotationVocabulary/>,
                               <https://spec.edmcouncil.org/fibo/ontology/master/latest/IND/Indicators/Indicators/>,
                               <https://spec.edmcouncil.org/fibo/ontology/master/latest/SEC/Equities/EquityInstruments/>,
                               <https://spec.edmcouncil.org/fibo/ontology/master/latest/SEC/Funds/Funds/>,
                               <https://spec.edmcouncil.org/fibo/ontology/master/latest/SEC/Securities/Pools/>,
                               <https://spec.edmcouncil.org/fibo/ontology/master/latest/SEC/Securities/SecuritiesClassification/>,
                               <https://spec.edmcouncil.org/fibo/ontology/master/latest/SEC/Securities/SecuritiesIdentification/>,
                               <https://spec.edmcouncil.org/fibo/ontology/master/latest/SEC/Securities/SecuritiesIssuance/>,
                               <https://spec.edmcouncil.org/fibo/ontology/master/latest/SEC/Securities/SecuritiesRestrictions/>,
                               <https://spec.edmcouncil.org/fibo/ontology/master/latest/SEC/Securities/SecurityAssets/>,
                               cmns-av:,
                               cmns-cls:,
                               cmns-col:,
                               cmns-cxtdsg:,
                               cmns-dt:,
                               cmns-dsg:,
                               cmns-doc:,
                               cmns-loc:,
                               cmns-org:,
                               cmns-pts:,
                               cmns-qtu:,
                               cmns-rga:,
                               cmns-rlcmp:,
                               <https://www.omg.org/spec/LCC/Countries/CountryRepresentation/>;
                   owl:versionIRI <https://spec.edmcouncil.org/fibo/ontology/master/latest/SEC/Funds/CollectiveInvestmentVehicles/>;
                   fibo-fnd-utl-av:hasMaturityLevel fibo-fnd-utl-av:Provisional;
                   cmns-av:copyright "Copyright (c) 2013-2025 EDM Council, Inc.",
                                     "Copyright (c) 2013-2025 Object Management Group, Inc.".
fibo-sec-fund-civ:AccumulatingShareClass a owl:Class;
                                         rdfs:isDefinedBy fibo-sec-fund-civ:;
                                         rdfs:label "accumulating share class"@en;
                                         rdfs:subClassOf fibo-sec-fund-civ:FundShareClassUnit;
                                         owl:disjointWith fibo-sec-fund-civ:DistributingShareClass;
                                         skos:definition "A share class in which there is no option to reinvest."@en;
                                         cmns-av:explanatoryNote "This fact would be determined by the fund unit having a specific Fund Distribution Policy of Accumulating."@en.
fibo-sec-fund-civ:AssetClassStrategy a owl:Class;
                                     rdfs:isDefinedBy fibo-sec-fund-civ:;
                                     rdfs:label "asset class strategy"@en;
                                     rdfs:subClassOf fibo-sec-fund-civ:FundPortfolioInvestmentLimitations,
                                                     [a owl:Restriction ; 
                                                      owl:onProperty fibo-sec-fund-civ:identifiesAssetTypesBy ; 
                                                      owl:someValuesFrom fibo-sec-sec-cls:FinancialInstrumentClassifier];
                                     skos:definition "Strategy which is asset class based."@en;
                                     cmns-av:explanatoryNote "EFAMA: The type of securities or other holdings that may be invested in. FIBIM: Strategy which is asset class based. Can implement this in terms of a classification of those things. Wording implies this is a policy."@en.
fibo-sec-fund-civ:CommonShareInFund a owl:Class;
                                    rdfs:isDefinedBy fibo-sec-fund-civ:;
                                    rdfs:label "common share in fund"@en;
                                    rdfs:subClassOf fibo-sec-fund-civ:FundShareClassUnit;
                                    owl:disjointWith fibo-sec-fund-civ:PreferredShareInFund;
                                    skos:definition "A share unit in a fund, which is classified as a Common Share class."@en;
                                    cmns-av:explanatoryNote "SR Review session notes: US: Closed and open ended funds may have common and preferred shares."@en.
fibo-sec-fund-civ:CurrencyStrategy a owl:Class;
                                   rdfs:isDefinedBy fibo-sec-fund-civ:;
                                   rdfs:label "currency strategy"@en;
                                   rdfs:subClassOf fibo-sec-fund-civ:FundPortfolioInvestmentLimitations;
                                   skos:definition "Strategy which is currency based."@en.
fibo-sec-fund-civ:DistributingShareClass a owl:Class;
                                         rdfs:isDefinedBy fibo-sec-fund-civ:;
                                         rdfs:label "distributing share class"@en;
                                         rdfs:subClassOf fibo-sec-fund-civ:FundShareClassUnit.
fibo-sec-fund-civ:EquityFund a owl:Class;
                             rdfs:isDefinedBy fibo-sec-fund-civ:;
                             rdfs:label "equity fund"@en;
                             rdfs:subClassOf fibo-sec-sec-pls:CollectiveInvestmentVehicle,
                                             [a owl:Restriction ; 
                                              owl:onProperty cmns-col:comprises ; 
                                              owl:someValuesFrom fibo-sec-fund-civ:EquityPortfolio];
                             skos:definition "A fund which invests in at least 85% shares."@en.
fibo-sec-fund-civ:EquityPortfolio a owl:Class;
                                  rdfs:isDefinedBy fibo-sec-fund-civ:;
                                  rdfs:label "equity portfolio"@en;
                                  rdfs:subClassOf fibo-sec-fund-civ:FundPortfolio,
                                                  [a owl:Restriction ; 
                                                   owl:onProperty cmns-col:comprises ; 
                                                   owl:someValuesFrom fibo-be-oac-cown:Shareholding];
                                  skos:definition "A portfolio which has at least 85% exposure to shares."@en.
fibo-sec-fund-civ:FondsCommunDePlacement a owl:Class;
                                         rdfs:isDefinedBy fibo-sec-fund-civ:;
                                         rdfs:label "fonds commun de placement"@fr-fr;
                                         rdfs:seeAlso <https://iclg.com/practice-areas/public-investment-funds-laws-and-regulations/france>,
                                                      <https://www.alfi.lu/en-gb/understandinginvesting/post/which-structure-to-choose>,
                                                      <https://www.ubp.com/en/glossary-risk-management/glossary-legal-compliance/fcp>;
                                         rdfs:subClassOf fibo-sec-sec-pls:CollectiveInvestmentVehicle;
                                         skos:definition "open-ended collective investment fund, which is a contractual form set up between the fund manager and investors and not a separate legal entity"@en;
                                         skos:note "An FCP is similar to a unit trust in the UK. FCPs are not investment companies, but more like open partnerships. They can be set up as a single fund or as an umbrella fund with multiple sub-funds, typically issued in the French-speaking countries of Europe."@en;
                                         cmns-av:abbreviation "FCP"@en.
fibo-sec-fund-civ:FundAccountant a owl:Class;
                                 rdfs:isDefinedBy fibo-sec-fund-civ:;
                                 rdfs:label "fund accountant"@en;
                                 rdfs:subClassOf fibo-sec-fund-civ:FundsProcessingParty;
                                 skos:definition "The party that keeps accounting records of the available assets and liabilities of the Fund. It calculates dealing prices, the Net Asset Value (NAV) of the Fund, and may provide fund performance and tax data. Can be subcontracted by the FundAdministrator."@en.
fibo-sec-fund-civ:FundBondClassUnit a owl:Class;
                                    rdfs:isDefinedBy fibo-sec-fund-civ:;
                                    rdfs:label "fund bond class unit"@en;
                                    rdfs:subClassOf fibo-sec-fund-fund:FundUnit,
                                                    [a owl:Restriction ; 
                                                     owl:onProperty fibo-fnd-gao-obj:hasStrategy ; 
                                                     owl:someValuesFrom fibo-sec-fund-civ:FundUnitDistributionPolicy],
                                                    [a owl:Restriction ; 
                                                     owl:onProperty fibo-sec-fund-civ:hasExpectedCoupon ; 
                                                     owl:someValuesFrom fibo-sec-fund-civ:FundBondUnitCoupon];
                                    skos:definition "A fund unit which takes the form of debt in that fund."@en;
                                    cmns-av:explanatoryNote "From EFAMA Review: called denominations e.g. issued in $5000 pieces. You cannot buy fractional amounts in a bond."@en.
fibo-sec-fund-civ:FundBondUnitCoupon a owl:Class;
                                     rdfs:isDefinedBy fibo-sec-fund-civ:;
                                     rdfs:label "fund bond unit coupon"@en;
                                     rdfs:subClassOf fibo-fnd-acc-cur:InterestRate,
                                                     [a owl:Restriction ; 
                                                      owl:onProperty fibo-sec-fund-civ:hasPolicyTerms ; 
                                                      owl:someValuesFrom fibo-sec-fund-civ:FundCouponPolicy];
                                     skos:definition "A fixed coupon paid out to holders of the Fund Bond Unit."@en.
fibo-sec-fund-civ:FundCashDistributionPolicy a owl:Class;
                                             rdfs:isDefinedBy fibo-sec-fund-civ:;
                                             rdfs:label "fund cash distribution policy"@en;
                                             rdfs:subClassOf fibo-sec-fund-civ:FundUnitDistributionPolicy;
                                             skos:definition """Policy for distribution of cash dividends or notes in the event that the fund units have a distribution policy of \"Cash\" rather than \"Reinvestment\"."""@en.
fibo-sec-fund-civ:FundClassification a owl:Class;
                                     rdfs:isDefinedBy fibo-sec-fund-civ:;
                                     rdfs:label "fund classification"@en;
                                     rdfs:subClassOf cmns-cls:Classifier,
                                                     [a owl:Restriction ; 
                                                      owl:onProperty cmns-cls:classifies ; 
                                                      owl:someValuesFrom fibo-sec-sec-pls:CollectiveInvestmentVehicle];
                                     skos:definition """The category of the fund according to the asset class. This is a published code by which the Fund is classified. Further notes: Could be EFCF codes. This is the way in which \"Type of fund\" is articulated."""@en.
fibo-sec-fund-civ:FundClassificationScheme a owl:Class;
                                           rdfs:isDefinedBy fibo-sec-fund-civ:;
                                           rdfs:label "fund classification scheme"@en;
                                           rdfs:subClassOf cmns-cls:ClassificationScheme,
                                                           [a owl:Restriction ; 
                                                            owl:onProperty cmns-dsg:defines ; 
                                                            owl:someValuesFrom fibo-sec-fund-civ:FundClassification];
                                           skos:definition "A published scheme for the category of a fund according to the asset class."@en.
fibo-sec-fund-civ:FundCouponPolicy a owl:Class;
                                   rdfs:isDefinedBy fibo-sec-fund-civ:;
                                   rdfs:label "fund coupon policy"@en;
                                   rdfs:subClassOf fibo-sec-fund-civ:FundCashDistributionPolicy;
                                   skos:definition "Terms for the expected distribution of bond unit coupons."@en.
fibo-sec-fund-civ:FundDepositary a owl:Class;
                                 rdfs:isDefinedBy fibo-sec-fund-civ:;
                                 rdfs:label "fund depositary"@en;
                                 rdfs:subClassOf fibo-sec-fund-civ:FundsProcessingParty,
                                                 [a owl:Restriction ; 
                                                  owl:onProperty fibo-sec-fund-civ:providesDepositaryServiceFor ; 
                                                  owl:someValuesFrom fibo-sec-fund-fund:FundUnit];
                                 skos:definition "The party that holds and safeguards holdings owned by a fund. It is also responsible for compliance of the portfolio with legal ratios etc."@en;
                                 cmns-av:explanatoryNote "The depository may delegate custody to another entity (custodian). Definition origin:EFAMA DD"@en.
fibo-sec-fund-civ:FundDistributionPolicy a owl:Class;
                                         rdfs:isDefinedBy fibo-sec-fund-civ:;
                                         rdfs:label "fund distribution policy"@en;
                                         rdfs:subClassOf fibo-fnd-law-lcap:Policy;
                                         skos:definition "policy indicating the overall strategy or limitations on distribution for the fund"@en;
                                         cmns-av:explanatoryNote """Note that individual classes of Fund Unit also have specific distribution polcies as they effect that class of unit. This class is for terms with wording of the form: \" ... whether or not it is possible to hold shares ...\" for a given parameter."""@en.
fibo-sec-fund-civ:FundDistributor a owl:Class;
                                  rdfs:isDefinedBy fibo-sec-fund-civ:;
                                  rdfs:label "fund distributor"@en;
                                  rdfs:subClassOf fibo-sec-fund-civ:FundsProcessingParty;
                                  skos:definition "an entity through which a fund may be bought by or for an investor. This may be on a discretionary or advisory basis, or as an execution-only service. Definition origin:EFAMA DD"@en.
fibo-sec-fund-civ:FundDividendPolicy a owl:Class;
                                     rdfs:isDefinedBy fibo-sec-fund-civ:;
                                     rdfs:label "fund dividend policy"@en;
                                     rdfs:subClassOf fibo-sec-fund-civ:FundCashDistributionPolicy;
                                     skos:definition "Terms for the expected distributions of dividends."@en.
fibo-sec-fund-civ:FundInvestmentObjective a owl:Class;
                                          rdfs:isDefinedBy fibo-sec-fund-civ:;
                                          rdfs:label "fund investment objective"@en;
                                          rdfs:subClassOf fibo-fnd-gao-obj:InvestmentObjective,
                                                          [a owl:Restriction ; 
                                                           owl:onProperty fibo-sec-fund-civ:hasIntendedRiskLevel ; 
                                                           owl:someValuesFrom fibo-sec-fund-civ:RiskLevel],
                                                          [a owl:Restriction ; 
                                                           owl:onProperty fibo-sec-fund-civ:statedIn ; 
                                                           owl:someValuesFrom fibo-sec-sec-iss:Prospectus];
                                          skos:definition "The aim of a Fund e.g outperfom a given benchmark."@en;
                                          skos:editorialNote "This could be broken down into other terms that can be itemised here, that are not in the EFAMA DD explicitly. Examples may include: - Risk level - Return - Exposure to different markets"@en.
fibo-sec-fund-civ:FundInvestmentPolicy a owl:Class;
                                       rdfs:isDefinedBy fibo-sec-fund-civ:;
                                       rdfs:label "fund investment policy"@en;
                                       rdfs:subClassOf fibo-fnd-law-lcap:Policy,
                                                       [a owl:Restriction ; 
                                                        owl:onProperty fibo-sec-fund-civ:stipulatesBenchmark ; 
                                                        owl:onClass fibo-ind-ind-ind:MarketRate ; 
                                                        owl:maxQualifiedCardinality "1"^^xsd:nonNegativeInteger],
                                                       [a owl:Restriction ; 
                                                        owl:onProperty cmns-dsg:defines ; 
                                                        owl:someValuesFrom fibo-sec-fund-civ:InvestmentRestriction],
                                                       [a owl:Restriction ; 
                                                        owl:onProperty cmns-rga:governs ; 
                                                        owl:someValuesFrom fibo-sec-fund-civ:PortfolioInvestmentStrategy];
                                       skos:definition "policy that the fund implements in order to achieve the stated fund objectives"@en;
                                       cmns-av:explanatoryNote """EFAMA Note: Model distinguishes between strategy (what you intend to invest in) and portfolio structure (what is held). This semantics matches the EFAMA DD \"Fund Investment Policy\" No stated definition in EFAMA DD (\"Further discussion required\")."""@en.
fibo-sec-fund-civ:FundLegalFormDocumentation a owl:Class;
                                             rdfs:isDefinedBy fibo-sec-fund-civ:;
                                             rdfs:label "fund legal form documentation"@en;
                                             rdfs:subClassOf fibo-fnd-law-cor:Constitution;
                                             skos:definition "For a fund which is constituted under the law of contract, the constitution or articles that define the fund. These are embodied in a Contract."@en;
                                             cmns-av:explanatoryNote """From ISO FIBIM \"Umbrella Fund\" narrative: In securities, a collective investment scheme that has a contractual or a corporate form. When it has a contractual form, a fund is constituted under either the law of contract or under the trust law and thus it is not a legal entity. In its corporate form, a fund is a legal entity and is structured as a company."""@en.
fibo-sec-fund-civ:FundOrderDesk a owl:Class;
                                rdfs:isDefinedBy fibo-sec-fund-civ:;
                                rdfs:label "fund order desk"@en;
                                rdfs:subClassOf fibo-fbc-pas-caa:AccountProvider,
                                                [a owl:Restriction ; 
                                                 owl:onProperty cmns-rlcmp:isPlayedBy ; 
                                                 owl:someValuesFrom cmns-org:LegalEntity];
                                skos:definition "The Fund Order Desk is a party to the Fund Order Desk Account."@en;
                                skos:editorialNote "This party would presumably be identified as the Fund Management Company in terms of what legal entity fulcils this role? to be determined at further review."@en.
fibo-sec-fund-civ:FundPortfolio a owl:Class;
                                rdfs:isDefinedBy fibo-sec-fund-civ:;
                                rdfs:label "fund portfolio"@en;
                                rdfs:subClassOf fibo-sec-sec-ast:Portfolio,
                                                [a owl:Restriction ; 
                                                 owl:onProperty fibo-fnd-acc-cur:hasMonetaryAmount ; 
                                                 owl:someValuesFrom fibo-fbc-pas-caa:Balance],
                                                [a owl:Restriction ; 
                                                 owl:onProperty fibo-sec-fund-civ:assessedAgainst ; 
                                                 owl:someValuesFrom fibo-sec-fund-civ:PortfolioBenchmark],
                                                [a owl:Restriction ; 
                                                 owl:onProperty fibo-sec-fund-civ:hasInvestmentStrategy ; 
                                                 owl:someValuesFrom fibo-sec-fund-civ:PortfolioInvestmentStrategy],
                                                [a owl:Restriction ; 
                                                 owl:onProperty fibo-sec-fund-civ:implementsFundPolicy ; 
                                                 owl:someValuesFrom fibo-sec-fund-civ:FundPortfolioInvestmentPolicy],
                                                [a owl:Restriction ; 
                                                 owl:onProperty cmns-col:comprises ; 
                                                 owl:someValuesFrom fibo-sec-sec-ast:Portfolio];
                                skos:definition "An account containing a number of financial instruments along with cash positions in one or more currencies and belonging to a Fund"@en.
fibo-sec-fund-civ:FundPortfolioInvestmentLimitations a owl:Class;
                                                     rdfs:isDefinedBy fibo-sec-fund-civ:;
                                                     rdfs:label "fund portfolio investment limitations"@en;
                                                     rdfs:subClassOf fibo-sec-fund-civ:InvestmentRestriction;
                                                     skos:definition "Detailed Policy on approximately how the portfolio is to be allocated to achieve the stated investment goals. This underpins the detailed strategy of how to achieve this."@en;
                                                     cmns-av:explanatoryNote """Defined as \"Strategy\" in FIBIM and elsewhere. WG11: Rough allocation of the portfolio."""@en.
fibo-sec-fund-civ:FundPortfolioInvestmentPolicy a owl:Class;
                                                rdfs:isDefinedBy fibo-sec-fund-civ:;
                                                rdfs:label "fund portfolio investment policy"@en;
                                                rdfs:subClassOf fibo-fnd-law-lcap:Policy,
                                                                [a owl:Restriction ; 
                                                                 owl:onProperty fibo-sec-fund-civ:definesAllocations ; 
                                                                 owl:someValuesFrom fibo-sec-fund-civ:FundPortfolioInvestmentLimitations],
                                                                [a owl:Restriction ; 
                                                                 owl:onProperty cmns-rga:governs ; 
                                                                 owl:someValuesFrom fibo-sec-fund-civ:PortfolioInvestmentStrategy];
                                                skos:definition "policy with respect to allocation of the portfolio that is designed to meet the stated investment strategy and goals"@en;
                                                cmns-av:explanatoryNote "ISO FIBIM: Rough allocation of the portfolio."@en.
fibo-sec-fund-civ:FundProcessingGeneralTerms a owl:Class;
                                             rdfs:isDefinedBy fibo-sec-fund-civ:;
                                             rdfs:label "fund processing general terms"@en;
                                             rdfs:subClassOf fibo-sec-fund-civ:FundProcessingTerms;
                                             skos:definition "Formal terms for general processing of the fund. These set out what the investor and the fund may or may not do."@en.
fibo-sec-fund-civ:FundProcessingTerms a owl:Class;
                                      rdfs:isDefinedBy fibo-sec-fund-civ:;
                                      rdfs:label "fund processing terms"@en;
                                      rdfs:subClassOf fibo-fnd-agr-ctr:ContractualCommitment,
                                                      [a owl:Restriction ; 
                                                       owl:onProperty fibo-sec-fund-civ:definesMainFundOrderDeskAccount ; 
                                                       owl:someValuesFrom fibo-sec-fund-civ:FundsProcessingAccount],
                                                      [a owl:Restriction ; 
                                                       owl:onProperty fibo-sec-fund-civ:hasDefaultSettlementConvention ; 
                                                       owl:someValuesFrom fibo-fbc-fi-stl:SettlementConvention];
                                      skos:definition "Formal terms for processing of the fund. These set out what the investor and the fund may or may not do. These include terms for redemption and subscription processing as well as general processing terms. ISO FIBIM definition: Processing characteristics linked to the instrument, ie, not to the market."@en;
                                      cmns-av:explanatoryNote "These include Fund Subscription Terms, Fund Redemption Terms. and terms which relate to general processing and restrictions or otherwise on the holder. FPP notes: FPP presentation identifies many of these terms under the heading of Valuation Dealing characteristics. May need to revise which goes where in line with FPP. See also terms under NAV Valuation Calculation Method. Others of these terms appear in FPP under Instrument Restrictions. These cover the subscription, redemption and holding amounts and units and minimum holding period."@en.
fibo-sec-fund-civ:FundRedemptionRestriction a owl:Class;
                                            rdfs:isDefinedBy fibo-sec-fund-civ:;
                                            rdfs:label "fund redemption restriction"@en;
                                            rdfs:subClassOf fibo-sec-sec-rst:SecuritiesRestriction.
fibo-sec-fund-civ:FundRedemptionTerms a owl:Class;
                                      rdfs:isDefinedBy fibo-sec-fund-civ:;
                                      rdfs:label "fund redemption terms"@en;
                                      rdfs:subClassOf fibo-sec-fund-civ:FundProcessingTerms,
                                                      [a owl:Restriction ; 
                                                       owl:onProperty fibo-sec-fund-civ:hasAdditionalRedemptionRestrictions ; 
                                                       owl:someValuesFrom fibo-sec-fund-civ:ReferToFundOrderDesk];
                                      skos:definition "Formal terms for redemption of units in the fund. These set out what the investor and the fund may or may not do."@en.
fibo-sec-fund-civ:FundReinvestmentPolicy a owl:Class;
                                         rdfs:isDefinedBy fibo-sec-fund-civ:;
                                         rdfs:label "fund reinvestment policy"@en;
                                         rdfs:subClassOf fibo-sec-fund-civ:FundUnitDistributionPolicy;
                                         skos:definition "Terms for the expected reinvestment of profits on fund units."@en.
fibo-sec-fund-civ:FundShareClassUnit a owl:Class;
                                     rdfs:isDefinedBy fibo-sec-fund-civ:;
                                     rdfs:label "fund share class unit"@en;
                                     rdfs:subClassOf fibo-sec-fund-fund:FundUnit,
                                                     [a owl:Restriction ; 
                                                      owl:onProperty fibo-fnd-gao-obj:hasStrategy ; 
                                                      owl:someValuesFrom fibo-sec-fund-civ:FundUnitDistributionPolicy];
                                     skos:definition "The legal structure in which you can purchase part of an investment pool, defined by a variety of characteristics like investor type, minimum size of investment, distribution type, fee and currency. A fund unit which gives the holder an equity stake in the fund."@en;
                                     cmns-av:explanatoryNote "From review sessions: Theoretically you can buy a fraction of a share in a fund. This would depend on the legal structure of the fund, e.g. a minimum investment. There is always a distribution plan."@en.
fibo-sec-fund-civ:FundSubscriptionTerms a owl:Class;
                                        rdfs:isDefinedBy fibo-sec-fund-civ:;
                                        rdfs:label "fund subscription terms"@en;
                                        rdfs:subClassOf fibo-sec-fund-civ:FundProcessingTerms,
                                                        [a owl:Restriction ; 
                                                         owl:onProperty cmns-cxtdsg:appliesTo ; 
                                                         owl:someValuesFrom fibo-sec-fund-fund:FundUnit];
                                        skos:definition "Subscription terms for the fund. Further notes: ISO FIBIM, EFAMA DD and FPP combine terms for subscription, redemption and general holding requirements. These have been separated here as they are different kinds of term, but this can be reviewed. Subscription Terms are identified as terms of the fund and not the fund unit, since terms for how you might subscribe can't be binding one someone who has not yet subscribed."@en.
fibo-sec-fund-civ:FundSupervisoryAuthority a owl:Class;
                                           rdfs:isDefinedBy fibo-sec-fund-civ:;
                                           rdfs:label "fund supervisory authority"@en;
                                           rdfs:subClassOf cmns-pts:PartyRole;
                                           skos:definition "party that supervises the fund or fund industry"@en.
fibo-sec-fund-civ:FundTransferAgent a owl:Class;
                                    rdfs:isDefinedBy fibo-sec-fund-civ:;
                                    rdfs:label "fund transfer agent"@en;
                                    rdfs:subClassOf fibo-sec-fund-civ:FundsProcessingParty;
                                    skos:definition "An entity that undertakes the execution of subscription, redemption and switch orders on behalf of a fund. Definition origin:EFAMA DD"@en.
fibo-sec-fund-civ:FundUnitDistributionMethod a owl:Class;
                                             rdfs:isDefinedBy fibo-sec-fund-civ:;
                                             rdfs:label "fund unit distribution method"@en;
                                             rdfs:subClassOf fibo-fnd-gao-obj:DistributionStrategy;
                                             skos:definition "The normal distribution policy for funds."@en.
fibo-sec-fund-civ:FundUnitDistributionPolicy a owl:Class;
                                             rdfs:isDefinedBy fibo-sec-fund-civ:;
                                             rdfs:label "fund unit distribution policy"@en;
                                             rdfs:subClassOf fibo-fnd-law-lcap:Policy,
                                                             [a owl:Restriction ; 
                                                              owl:onProperty fibo-fnd-gao-obj:hasStrategy ; 
                                                              owl:someValuesFrom fibo-sec-fund-civ:FundUnitDistributionMethod];
                                             skos:definition "policy relating to the unit, e.g. if income is paid out or retained in the fund and how this is treated, including distribution policy details for dividends and coupons."@en.
fibo-sec-fund-civ:FundsCashDistribution a owl:Class;
                                        rdfs:isDefinedBy fibo-sec-fund-civ:;
                                        rdfs:label "funds cash distribution"@en;
                                        rdfs:subClassOf fibo-sec-fund-civ:FundUnitDistributionMethod;
                                        skos:definition "Accrued income is distributed periodically to the investor."@en.
fibo-sec-fund-civ:FundsProcessing a owl:Class;
                                  rdfs:isDefinedBy fibo-sec-fund-civ:;
                                  rdfs:label "funds processing"@en;
                                  rdfs:subClassOf fibo-fnd-arr-lif:LifecycleStage;
                                  skos:definition "The context of managing and processing funds, issuing funds units etc. This is the context in which the different parties involved in a fund are defined as parties."@en.
fibo-sec-fund-civ:FundsProcessingAccount a owl:Class;
                                         rdfs:isDefinedBy fibo-sec-fund-civ:;
                                         rdfs:label "funds processing account"@en;
                                         rdfs:subClassOf fibo-fbc-pas-caa:Account,
                                                         [a owl:Restriction ; 
                                                          owl:onProperty cmns-org:isProvidedBy ; 
                                                          owl:someValuesFrom fibo-sec-fund-civ:FundOrderDesk];
                                         skos:definition "An account used specifically in the processing of funds. Like all accounts this is (per FIBIM definition) a business relationship between two entities; one entity is the account owner, the other entity is the account servicer. Please refer to Financial global model for treatment of accounts relationships in this model."@en;
                                         cmns-av:explanatoryNote """Derived from FIBIM definition for \"Account\", which is: \"Business relationship between two entities; one entity is the account owner, the other entity is the account servicer.\" this corresponds to the Global Terms definition for Account."""@en.
fibo-sec-fund-civ:FundsProcessingParty a owl:Class;
                                       rdfs:isDefinedBy fibo-sec-fund-civ:;
                                       rdfs:label "funds processing party"@en;
                                       rdfs:subClassOf cmns-pts:PartyRole;
                                       skos:definition "party involved in the processing of funds"@en.
fibo-sec-fund-civ:IncomeAccumulation a owl:Class;
                                     rdfs:isDefinedBy fibo-sec-fund-civ:;
                                     rdfs:label "income accumulation"@en;
                                     rdfs:subClassOf fibo-sec-fund-civ:FundUnitDistributionMethod;
                                     skos:definition "Accrued income is not distributed and instead remains reflected within the unit/share price."@en.
fibo-sec-fund-civ:InvestmentRestriction a owl:Class;
                                        rdfs:isDefinedBy fibo-sec-fund-civ:;
                                        rdfs:label "fund investment restrictions set"@en;
                                        rdfs:subClassOf fibo-sec-sec-rst:SecuritiesRestriction,
                                                        [a owl:Restriction ; 
                                                         owl:onProperty cmns-col:isPartOf ; 
                                                         owl:someValuesFrom fibo-sec-sec-iss:Prospectus];
                                        skos:definition "Limitations that apply to the fund as a whole, such as risk factors. these are used to determine whether the fund is appropriate for a given type of investor to invest in."@en;
                                        cmns-av:explanatoryNote "These are defined by the overall Fund investment policy. Not the same as the detailed policies for investing in percentages of this or that."@en.
fibo-sec-fund-civ:InvestmentStrategy a owl:Class;
                                     rdfs:isDefinedBy fibo-sec-fund-civ:;
                                     rdfs:label "investment strategy"@en;
                                     rdfs:subClassOf fibo-fnd-gao-obj:BusinessStrategy,
                                                     [a owl:Restriction ; 
                                                      owl:onProperty fibo-fnd-gao-obj:hasObjective ; 
                                                      owl:someValuesFrom fibo-fnd-gao-obj:InvestmentObjective];
                                     skos:definition "plan, method, or series of maneuvers or stratagems for obtaining a specific investment goal"@en.
fibo-sec-fund-civ:JurisdictionStrategy a owl:Class;
                                       rdfs:isDefinedBy fibo-sec-fund-civ:;
                                       rdfs:label "jurisdiction strategy"@en;
                                       rdfs:subClassOf fibo-sec-fund-civ:FundPortfolioInvestmentLimitations,
                                                       [a owl:Restriction ; 
                                                        owl:onProperty cmns-cxtdsg:isApplicableIn ; 
                                                        owl:someValuesFrom cmns-rga:Jurisdiction];
                                       skos:definition "Strategy which is jurisdiction based."@en.
fibo-sec-fund-civ:KeyInvestorInformationDocument a owl:Class;
                                                 rdfs:isDefinedBy fibo-sec-fund-civ:;
                                                 rdfs:label "key investor information document";
                                                 rdfs:subClassOf fibo-sec-sec-iss:OfferingDocument,
                                                                 [a owl:Restriction ; 
                                                                  owl:onProperty cmns-cxtdsg:isApplicableIn ; 
                                                                  owl:hasValue fibo-be-ge-euj:EuropeanUnionJurisdiction],
                                                                 [a owl:Restriction ; 
                                                                  owl:onProperty cmns-cxtdsg:appliesTo ; 
                                                                  owl:someValuesFrom fibo-sec-fund-fund:FundUnit];
                                                 skos:definition "short document that provides critical information for investors, summarizing content derived from a prospectus such that it can be understood by investors without reference to other documents, as required by law in the European Union";
                                                 cmns-av:abbreviation "KIID";
                                                 cmns-av:adaptedFrom "https://eur-lex.europa.eu/eli/dir/2009/65/2020-01-07"^^xsd:anyURI;
                                                 cmns-av:explanatoryNote "Key investor information shall include appropriate information about the essential characteristics of the UCITS concerned, which is to be provided to investors so that they are reasonably able to understand the nature and the risks of the investment product that is being offered to them and, consequently, to take investment decisions on an informed basis.".
fibo-sec-fund-civ:NetAssetValueCalculationMethod a owl:Class;
                                                 rdfs:isDefinedBy fibo-sec-fund-civ:;
                                                 rdfs:label "net asset value calculation method"@en;
                                                 rdfs:subClassOf cmns-qtu:Expression,
                                                                 [a owl:Restriction ; 
                                                                  owl:onProperty fibo-sec-fund-civ:isCalculatedIn ; 
                                                                  owl:someValuesFrom fibo-fnd-acc-cur:Currency];
                                                 skos:definition "Parameters for the calculation of the net asset value for an investment fund/fund class."@en;
                                                 skos:editorialNote "These terms were in the ISO FIBIM model but correspond to some details in the EFAMA DD."@en.
fibo-sec-fund-civ:NoteFund a owl:Class;
                           rdfs:isDefinedBy fibo-sec-fund-civ:;
                           rdfs:label "note fund";
                           rdfs:subClassOf fibo-sec-sec-pls:ManagedInvestment;
                           skos:definition "pooled investment vehicle that issues debt instruments (notes) to investors rather than (or in addition to) traditional equity interests";
                           cmns-av:explanatoryNote "The notes issued by a note fund are typically privately rated by agencies like KBRA, DBRS, or Moody's, tranched into senior and junior classes, and linked to underlying assets such as private loans, credit instruments, or structured products. Note funds are designed to optimize regulatory capital treatment, especially for insurance companies, by offering rated debt instead of equity.".
fibo-sec-fund-civ:NoteFundShare a owl:Class;
                                rdfs:isDefinedBy fibo-sec-fund-civ:;
                                rdfs:label "note fund share";
                                rdfs:subClassOf fibo-sec-fund-fund:FundUnit,
                                                [a owl:Restriction ; 
                                                 owl:onProperty cmns-col:isPartOf ; 
                                                 owl:someValuesFrom fibo-sec-fund-civ:NoteFund];
                                skos:definition "investment interest in a fund that issues notes rather than traditional equity, in cases where the fund is structured as a company";
                                cmns-av:explanatoryNote "A note fund share refers to an equity or debt-linked interest in a corporate fund vehicle that issues notes.".
fibo-sec-fund-civ:NoteFundUnit a owl:Class;
                               rdfs:isDefinedBy fibo-sec-fund-civ:;
                               rdfs:label "note fund unit";
                               rdfs:subClassOf fibo-sec-fund-fund:FundUnit,
                                               [a owl:Restriction ; 
                                                owl:onProperty cmns-col:isPartOf ; 
                                                owl:someValuesFrom fibo-sec-fund-civ:NoteFund];
                               skos:definition "investment interest in a fund that issues notes rather than traditional equity, in cases where the fund is structured as a trust, partnership, or unitized fund";
                               cmns-av:explanatoryNote "A note fund unit refers to a non-equity interest in a fund that issues rated notes and is organized as a unit trust or limited partnership.".
fibo-sec-fund-civ:OrganizationStrategy a owl:Class;
                                       rdfs:isDefinedBy fibo-sec-fund-civ:;
                                       rdfs:label "organization strategy"@en;
                                       rdfs:subClassOf fibo-sec-fund-civ:FundPortfolioInvestmentLimitations,
                                                       [a owl:Restriction ; 
                                                        owl:onProperty fibo-sec-fund-civ:definedInRelationTo ; 
                                                        owl:someValuesFrom fibo-be-le-cb:Corporation];
                                       skos:definition "Strategy which is organization based."@en.
fibo-sec-fund-civ:OtherInvestmentFundInformation a owl:Class;
                                                 rdfs:isDefinedBy fibo-sec-fund-civ:;
                                                 rdfs:label "other investment fund information"@en;
                                                 rdfs:subClassOf cmns-doc:Document;
                                                 skos:definition "Things which are not part of the prospectus but are important if you want to understand the fund."@en;
                                                 skos:editorialNote """See terms in EFAMA spreadsheet. These are properties of the fund but are not legally binding. Author follow-up note: I have managed to find a \"home\" for disposition for most of the entries that are in the spreadsheet. It is not clear which of the spreadsheet terms are indended to come under the general heading in this class. The first place I would look is in the terms I have defined as \"Fund Processing Terms\", which are defined as formal, legal contractual terms. If any of those are not legally binding on some party, then this is where they belong instead."""@en.
fibo-sec-fund-civ:PortfolioBenchmark a owl:Class;
                                     rdfs:isDefinedBy fibo-sec-fund-civ:;
                                     rdfs:label "portfolio benchmark"@en;
                                     rdfs:subClassOf cmns-qtu:Measure,
                                                     [a owl:Restriction ; 
                                                      owl:onProperty fibo-sec-fund-civ:definesBenchmark ; 
                                                      owl:someValuesFrom fibo-ind-ind-ind:MarketRate],
                                                     [a owl:Restriction ; 
                                                      owl:onProperty cmns-cxtdsg:appliesTo ; 
                                                      owl:someValuesFrom fibo-sec-fund-civ:FundPortfolio];
                                     skos:definition "Security or other price against which the performance of the portfolio is evaluated."@en.
fibo-sec-fund-civ:PortfolioInvestmentStrategy a owl:Class;
                                              rdfs:isDefinedBy fibo-sec-fund-civ:;
                                              rdfs:label "portfolio investment strategy"@en;
                                              rdfs:subClassOf fibo-sec-fund-civ:InvestmentStrategy,
                                                              [a owl:Restriction ; 
                                                               owl:onProperty cmns-col:comprises ; 
                                                               owl:someValuesFrom fibo-sec-fund-civ:FundPortfolioInvestmentLimitations];
                                              skos:definition "The manner in which the portfolio manager tries to reach the funds objectives."@en;
                                              cmns-av:explanatoryNote """Describes how you get there. E.g fully invested v not fully invested. MB Note: The terms labeled \"Strategy\" in EFAMA and in FIBIM are more like dictionary definition of policy, while \"How you get there\" is a dictionary definition of Strategy. Therefore original labels may be reversed from dictionary definition of the global semantics these are derived from."""@en.
fibo-sec-fund-civ:PreferredShareInFund a owl:Class;
                                       rdfs:isDefinedBy fibo-sec-fund-civ:;
                                       rdfs:label "preferred share in fund"@en;
                                       rdfs:subClassOf fibo-sec-fund-civ:FundShareClassUnit.
fibo-sec-fund-civ:PrivateEquityHolding a owl:Class;
                                       rdfs:isDefinedBy fibo-sec-fund-civ:;
                                       rdfs:label "private equity holding"@en;
                                       rdfs:subClassOf fibo-sec-sec-ast:Portfolio,
                                                       [a owl:Restriction ; 
                                                        owl:onProperty cmns-col:comprises ; 
                                                        owl:someValuesFrom fibo-sec-eq-eq:PrivatelyHeldShare];
                                       skos:definition "A holding of private equity."@en.
fibo-sec-fund-civ:RealEstateHolding a owl:Class;
                                    rdfs:isDefinedBy fibo-sec-fund-civ:;
                                    rdfs:label "real estate holding"@en;
                                    rdfs:subClassOf fibo-sec-sec-ast:Portfolio,
                                                    [a owl:Restriction ; 
                                                     owl:onProperty cmns-col:comprises ; 
                                                     owl:someValuesFrom fibo-fnd-plc-rp:RealEstate];
                                    skos:definition "tangible asset consisting of real estate that is owned or controlled by an individual, organization, or entity for investment, operational, or strategic purposes"@en.
fibo-sec-fund-civ:ReferToFundOrderDesk a owl:Class;
                                       rdfs:isDefinedBy fibo-sec-fund-civ:;
                                       rdfs:label "refer to fund order desk"@en;
                                       rdfs:subClassOf fibo-sec-fund-civ:FundRedemptionRestriction;
                                       skos:definition "Restriction requiring an investor to refer to the fund order desk prior to redeeming a fund."@en;
                                       skos:editorialNote "While it's unclear from original data models, it's likely that this restriction is actually to learn from the fund order desk of any other individual kinds of restriction that will apply. This is itself treated as a kind of restriction here."@en.
fibo-sec-fund-civ:RiskLevel a owl:Class;
                            rdfs:isDefinedBy fibo-sec-fund-civ:;
                            rdfs:label "risk level"@en;
                            rdfs:subClassOf cmns-cls:Classifier.
fibo-sec-fund-civ:SICAF a owl:Class;
                        rdfs:isDefinedBy fibo-sec-fund-civ:;
                        rdfs:label "s i c a f"@en;
                        rdfs:subClassOf fibo-sec-sec-pls:CollectiveInvestmentVehicle;
                        skos:definition "A French fund vehicle type. Designation and definition needed."@en.
fibo-sec-fund-civ:SICAV a owl:Class;
                        rdfs:isDefinedBy fibo-sec-fund-civ:;
                        rdfs:label "s i c a v"@en;
                        rdfs:subClassOf fibo-sec-sec-pls:CollectiveInvestmentVehicle;
                        skos:definition "Societe Collective a Capital Variable"@en.
fibo-sec-fund-civ:SectorStrategy a owl:Class;
                                 rdfs:isDefinedBy fibo-sec-fund-civ:;
                                 rdfs:label "sector strategy"@en;
                                 rdfs:subClassOf fibo-sec-fund-civ:FundPortfolioInvestmentLimitations;
                                 skos:definition "Strategy which is sector based."@en.
fibo-sec-fund-civ:UnitIssuer a owl:Class;
                             rdfs:isDefinedBy fibo-sec-fund-civ:;
                             rdfs:label "unit issuer"@en;
                             rdfs:subClassOf fibo-sec-fund-civ:FundsProcessingParty,
                                             [a owl:Restriction ; 
                                              owl:onProperty fibo-fnd-rel-rel:issues ; 
                                              owl:someValuesFrom fibo-sec-fund-fund:FundUnit],
                                             [a owl:Restriction ; 
                                              owl:onProperty cmns-rlcmp:isPlayedBy ; 
                                              owl:someValuesFrom fibo-be-le-cb:Corporation];
                             skos:definition "The party which issues the Fund Unit."@en.
fibo-sec-fund-civ:accountingYearEndDate a owl:ObjectProperty;
                                        rdfs:isDefinedBy fibo-sec-fund-civ:;
                                        rdfs:label "accounting year end date"@en;
                                        rdfs:range fibo-fnd-dt-bd:DayOfMonth;
                                        skos:definition "Last day of the accounting year for the fund."@en.
fibo-sec-fund-civ:additionalRestrictions a owl:DatatypeProperty;
                                         rdfs:domain fibo-sec-fund-civ:OrganizationStrategy;
                                         rdfs:isDefinedBy fibo-sec-fund-civ:;
                                         rdfs:label "additional restrictions"@en;
                                         rdfs:range xsd:string;
                                         skos:definition "Other restrictions or treatment information in respect of this strategy and the organization to which it refers."@en.
fibo-sec-fund-civ:administeredBy a owl:ObjectProperty;
                                 rdfs:domain fibo-sec-sec-pls:CollectiveInvestmentVehicle;
                                 rdfs:isDefinedBy fibo-sec-fund-civ:;
                                 rdfs:label "administered by"@en;
                                 rdfs:range fibo-sec-fund-fund:FundAdministrator;
                                 rdfs:subPropertyOf fibo-sec-fund-civ:fundHasRelatedParty.
fibo-sec-fund-civ:advisedBy a owl:ObjectProperty;
                            rdfs:domain fibo-sec-sec-pls:CollectiveInvestmentVehicle;
                            rdfs:isDefinedBy fibo-sec-fund-civ:;
                            rdfs:label "advised by"@en;
                            rdfs:range fibo-fbc-fct-fse:RegisteredInvestmentAdvisor;
                            rdfs:subPropertyOf fibo-sec-fund-civ:fundHasRelatedParty.
fibo-sec-fund-civ:assessedAgainst a owl:ObjectProperty;
                                  rdfs:domain fibo-sec-fund-civ:FundPortfolio;
                                  rdfs:isDefinedBy fibo-sec-fund-civ:;
                                  rdfs:label "assessed against"@en;
                                  rdfs:range fibo-sec-fund-civ:PortfolioBenchmark.
fibo-sec-fund-civ:authorizedCountry a owl:ObjectProperty;
                                    rdfs:domain fibo-sec-fund-civ:FundProcessingGeneralTerms;
                                    rdfs:isDefinedBy fibo-sec-fund-civ:;
                                    rdfs:label "authorized country"@en;
                                    rdfs:range cmns-loc:Country;
                                    skos:definition "Country in which it is authorised to commercialise the fund."@en.
fibo-sec-fund-civ:backEndLoadApplicable a owl:DatatypeProperty;
                                        rdfs:domain fibo-sec-fund-civ:FundProcessingGeneralTerms;
                                        rdfs:isDefinedBy fibo-sec-fund-civ:;
                                        rdfs:label "back end load applicable"@en;
                                        rdfs:range xsd:boolean;
                                        skos:definition "Whether an exit charge, eg, CDSC, on redemption orders for this class can be applied."@en.
fibo-sec-fund-civ:benchmarkWeight a owl:ObjectProperty;
                                  rdfs:domain fibo-sec-fund-civ:PortfolioBenchmark;
                                  rdfs:isDefinedBy fibo-sec-fund-civ:;
                                  rdfs:label "benchmark weight"@en;
                                  rdfs:range cmns-qtu:Percentage;
                                  skos:definition "Instrument weighting in the benchmark for the portfolio."@en.
fibo-sec-fund-civ:blacklisted a owl:DatatypeProperty;
                              rdfs:domain fibo-sec-fund-civ:OrganizationStrategy;
                              rdfs:isDefinedBy fibo-sec-fund-civ:;
                              rdfs:label "blacklisted"@en;
                              rdfs:range xsd:boolean;
                              skos:definition "Whether or not the strategy in framed so as to include the referenced business entity as being blacklisted. If yes, the strategy prevents investment in securities issued by that organization."@en.
fibo-sec-fund-civ:clearFundsRequired a owl:DatatypeProperty;
                                     rdfs:domain fibo-fbc-pas-fpas:SettlementTerms;
                                     rdfs:isDefinedBy fibo-sec-fund-civ:;
                                     rdfs:label "clear funds required"@en;
                                     rdfs:range xsd:boolean;
                                     skos:definition "Whether cleared funds may be required before a subscription order can be executed."@en.
fibo-sec-fund-civ:couponPaymentDate a owl:ObjectProperty;
                                    rdfs:domain fibo-sec-fund-civ:FundCouponPolicy;
                                    rdfs:isDefinedBy fibo-sec-fund-civ:;
                                    rdfs:label "coupon payment date"@en;
                                    rdfs:range fibo-fnd-dt-bd:DayOfMonth;
                                    skos:definition "The date at which the coupon is distributed to the bond unit holder."@en.
fibo-sec-fund-civ:dealingFrequencyDescription a owl:DatatypeProperty;
                                              rdfs:domain fibo-sec-fund-civ:FundProcessingTerms;
                                              rdfs:isDefinedBy fibo-sec-fund-civ:;
                                              rdfs:label "dealing frequency description"@en;
                                              rdfs:range xsd:string;
                                              skos:definition "Description of frequency at which the subscriptions and redemptions are done."@en.
fibo-sec-fund-civ:declarationChannel a owl:DatatypeProperty;
                                     rdfs:domain fibo-sec-fund-civ:NetAssetValueCalculationMethod;
                                     rdfs:isDefinedBy fibo-sec-fund-civ:;
                                     rdfs:label "declaration channel"@en;
                                     rdfs:range xsd:string;
                                     skos:definition "Means of the net asset value publication, eg, a newspaper."@en.
fibo-sec-fund-civ:definedInRelationTo a owl:ObjectProperty;
                                      rdfs:domain fibo-sec-fund-civ:OrganizationStrategy;
                                      rdfs:isDefinedBy fibo-sec-fund-civ:;
                                      rdfs:label "defined in relation to"@en;
                                      rdfs:range fibo-be-le-cb:Corporation.
fibo-sec-fund-civ:definesAllocations a owl:ObjectProperty;
                                     rdfs:domain fibo-sec-fund-civ:FundPortfolioInvestmentPolicy;
                                     rdfs:isDefinedBy fibo-sec-fund-civ:;
                                     rdfs:label "defines allocations"@en;
                                     rdfs:range fibo-sec-fund-civ:FundPortfolioInvestmentLimitations;
                                     rdfs:subPropertyOf cmns-dsg:defines.
fibo-sec-fund-civ:definesBenchmark a owl:ObjectProperty;
                                   rdfs:domain fibo-sec-fund-civ:PortfolioBenchmark;
                                   rdfs:isDefinedBy fibo-sec-fund-civ:;
                                   rdfs:label "defines benchmark"@en;
                                   rdfs:range fibo-ind-ind-ind:MarketRate.
fibo-sec-fund-civ:definesMainFundOrderDeskAccount a owl:ObjectProperty;
                                                  rdfs:domain fibo-sec-fund-civ:FundProcessingTerms;
                                                  rdfs:isDefinedBy fibo-sec-fund-civ:;
                                                  rdfs:label "defines main fund order desk account"@en;
                                                  rdfs:range fibo-sec-fund-civ:FundsProcessingAccount.
fibo-sec-fund-civ:distributedBy a owl:ObjectProperty;
                                rdfs:domain fibo-sec-sec-pls:CollectiveInvestmentVehicle;
                                rdfs:isDefinedBy fibo-sec-fund-civ:;
                                rdfs:label "distributed by"@en;
                                rdfs:range fibo-sec-fund-civ:FundDistributor;
                                rdfs:subPropertyOf fibo-sec-fund-civ:fundHasRelatedParty.
fibo-sec-fund-civ:distributionWithReinvestment a owl:DatatypeProperty;
                                               rdfs:domain fibo-sec-fund-civ:FundReinvestmentPolicy,
                                                           fibo-sec-fund-civ:FundUnitDistributionPolicy;
                                               rdfs:isDefinedBy fibo-sec-fund-civ:;
                                               rdfs:label "distribution with reinvestment"@en;
                                               rdfs:range xsd:boolean;
                                               skos:definition "It is possible to hold shares for which the accrued income is distributed, but then reinvested automatically in additional units/shares allocated to the investor."@en.
fibo-sec-fund-civ:dualFund a owl:DatatypeProperty;
                           rdfs:domain fibo-sec-fund-civ:FundProcessingGeneralTerms;
                           rdfs:isDefinedBy fibo-sec-fund-civ:;
                           rdfs:label "dual fund"@en;
                           rdfs:range xsd:boolean;
                           skos:definition "Whether the fund has two prices."@en.
fibo-sec-fund-civ:endOfFiscalYear a owl:ObjectProperty;
                                  rdfs:isDefinedBy fibo-sec-fund-civ:;
                                  rdfs:label "end of fiscal year"@en;
                                  rdfs:range fibo-fnd-dt-bd:DayOfMonth;
                                  skos:definition "Day and month on any given year at which the books are closed and profit and loss is determined."@en.
fibo-sec-fund-civ:exCouponDate a owl:ObjectProperty;
                               rdfs:domain fibo-sec-fund-civ:FundCouponPolicy;
                               rdfs:isDefinedBy fibo-sec-fund-civ:;
                               rdfs:label "ex coupon date"@en;
                               rdfs:range fibo-fnd-dt-bd:DayOfMonth;
                               skos:definition "The date at which the coupon is substracted from the NAV"@en.
fibo-sec-fund-civ:firstAccountingYearEndDate a owl:DatatypeProperty;
                                             rdfs:isDefinedBy fibo-sec-fund-civ:;
                                             rdfs:label "first accounting year end date"@en;
                                             skos:definition "Last day of the first accounting year for the fund."@en.
fibo-sec-fund-civ:firstNAVCalculationDate a owl:DatatypeProperty;
                                          rdfs:domain fibo-sec-sec-pls:CollectiveInvestmentVehicle;
                                          rdfs:isDefinedBy fibo-sec-fund-civ:;
                                          rdfs:label "first n a v calculation date"@en;
                                          skos:definition "The first date of NAV calculation"@en.
fibo-sec-fund-civ:frontEndLoadApplicable a owl:DatatypeProperty;
                                         rdfs:domain fibo-sec-fund-civ:FundSubscriptionTerms;
                                         rdfs:isDefinedBy fibo-sec-fund-civ:;
                                         rdfs:label "front end load applicable"@en;
                                         rdfs:range xsd:boolean;
                                         skos:definition "Whether a front end charge on subscription orders for this class can be applied."@en.
fibo-sec-fund-civ:fundClassTypeIdentifier a owl:DatatypeProperty;
                                          rdfs:domain fibo-sec-fund-fund:FundUnit;
                                          rdfs:isDefinedBy fibo-sec-fund-civ:;
                                          rdfs:label "fund class type identifier"@en;
                                          rdfs:range xsd:string;
                                          skos:definition "A textual identification of the class of fund units. This is used to uniquely identify a particular class of fund units, and thereby identify features of this type of unit within the fund."@en.
fibo-sec-fund-civ:fundHasRelatedParty a owl:ObjectProperty;
                                      rdfs:domain fibo-sec-sec-pls:CollectiveInvestmentVehicle;
                                      rdfs:isDefinedBy fibo-sec-fund-civ:;
                                      rdfs:label "fund has related party"@en;
                                      rdfs:range fibo-sec-fund-civ:FundsProcessingParty.
fibo-sec-fund-civ:hasAdditionalInformation a owl:ObjectProperty;
                                           rdfs:domain fibo-sec-sec-pls:CollectiveInvestmentVehicle;
                                           rdfs:isDefinedBy fibo-sec-fund-civ:;
                                           rdfs:label "has additional information"@en;
                                           rdfs:range fibo-sec-fund-civ:OtherInvestmentFundInformation.
fibo-sec-fund-civ:hasAdditionalRedemptionRestrictions a owl:ObjectProperty;
                                                      rdfs:domain fibo-sec-fund-civ:FundRedemptionTerms;
                                                      rdfs:isDefinedBy fibo-sec-fund-civ:;
                                                      rdfs:label "has additional redemption restrictions"@en;
                                                      rdfs:range fibo-sec-fund-civ:ReferToFundOrderDesk.
fibo-sec-fund-civ:hasAuditor a owl:ObjectProperty;
                             rdfs:domain fibo-sec-sec-pls:CollectiveInvestmentVehicle;
                             rdfs:isDefinedBy fibo-sec-fund-civ:;
                             rdfs:label "has auditor"@en;
                             rdfs:range fibo-be-oac-exec:ExternalAuditor;
                             rdfs:subPropertyOf fibo-sec-fund-civ:fundHasRelatedParty.
fibo-sec-fund-civ:hasDataProvider a owl:ObjectProperty;
                                  rdfs:domain fibo-sec-sec-pls:CollectiveInvestmentVehicle;
                                  rdfs:isDefinedBy fibo-sec-fund-civ:;
                                  rdfs:label "has data provider"@en;
                                  rdfs:range fibo-be-fct-pub:MarketDataProvider;
                                  rdfs:subPropertyOf fibo-sec-fund-civ:fundHasRelatedParty;
                                  skos:definition "has an organization which is the data provider and is legally responsible for the information provided"@en.
fibo-sec-fund-civ:hasDefaultSettlementConvention a owl:ObjectProperty;
                                                 rdfs:domain fibo-sec-fund-civ:FundProcessingTerms;
                                                 rdfs:isDefinedBy fibo-sec-fund-civ:;
                                                 rdfs:label "has default settlement convention"@en;
                                                 rdfs:range fibo-fbc-fi-stl:SettlementConvention.
fibo-sec-fund-civ:hasDepository a owl:ObjectProperty;
                                rdfs:domain fibo-sec-sec-pls:CollectiveInvestmentVehicle;
                                rdfs:isDefinedBy fibo-sec-fund-civ:;
                                rdfs:label "has depository"@en;
                                rdfs:range fibo-sec-fund-civ:FundDepositary;
                                rdfs:subPropertyOf fibo-sec-fund-civ:fundHasRelatedParty.
fibo-sec-fund-civ:hasDetails a owl:ObjectProperty;
                             rdfs:domain fibo-sec-fund-fund:FundUnit;
                             rdfs:isDefinedBy fibo-sec-fund-civ:;
                             rdfs:label "has details"@en;
                             rdfs:range fibo-sec-fund-civ:NetAssetValueCalculationMethod;
                             skos:definition "Information on the net asset value calculation of the investment fund component."@en.
fibo-sec-fund-civ:hasExpectedCoupon a owl:ObjectProperty;
                                    rdfs:domain fibo-sec-fund-civ:FundBondClassUnit;
                                    rdfs:isDefinedBy fibo-sec-fund-civ:;
                                    rdfs:label "has expected coupon"@en;
                                    rdfs:range fibo-sec-fund-civ:FundBondUnitCoupon.
fibo-sec-fund-civ:hasFundPolicy a owl:ObjectProperty;
                                rdfs:domain fibo-sec-sec-pls:CollectiveInvestmentVehicle;
                                rdfs:isDefinedBy fibo-sec-fund-civ:;
                                rdfs:label "has fund policy"@en;
                                rdfs:range fibo-sec-fund-civ:FundInvestmentPolicy;
                                skos:definition "Overall policy for amounts invested, limitations etc. Not the same as the detailed Portfolio policy."@en.
fibo-sec-fund-civ:hasFundProcessingTerms a owl:ObjectProperty;
                                         rdfs:domain fibo-sec-fund-fund:FundUnit;
                                         rdfs:isDefinedBy fibo-sec-fund-civ:;
                                         rdfs:label "has fund processing terms"@en;
                                         rdfs:range fibo-sec-fund-civ:FundProcessingTerms;
                                         rdfs:subPropertyOf fibo-fnd-agr-ctr:hasContractualElement.
fibo-sec-fund-civ:hasIntendedRiskLevel a owl:ObjectProperty;
                                       rdfs:domain fibo-sec-fund-civ:FundInvestmentObjective;
                                       rdfs:isDefinedBy fibo-sec-fund-civ:;
                                       rdfs:label "has intended risk level"@en;
                                       rdfs:range fibo-sec-fund-civ:RiskLevel.
fibo-sec-fund-civ:hasInvestmentStrategy a owl:ObjectProperty;
                                        rdfs:domain fibo-sec-sec-ast:Portfolio;
                                        rdfs:isDefinedBy fibo-sec-fund-civ:;
                                        rdfs:label "strategy"@en;
                                        rdfs:range fibo-sec-fund-civ:InvestmentStrategy.
fibo-sec-fund-civ:hasIssueDate a owl:ObjectProperty;
                               rdfs:domain fibo-sec-fund-fund:FundUnit;
                               rdfs:isDefinedBy fibo-sec-fund-civ:;
                               rdfs:label "has issue date"@en;
                               rdfs:range cmns-dt:Date;
                               skos:definition "Date of first NAV calculation and start of performance calculations (same as launch date)"@en.
fibo-sec-fund-civ:hasManagementCompany a owl:ObjectProperty;
                                       rdfs:domain fibo-sec-sec-pls:CollectiveInvestmentVehicle;
                                       rdfs:isDefinedBy fibo-sec-fund-civ:;
                                       rdfs:label "has management company"@en;
                                       rdfs:range fibo-sec-fund-fund:FundManager;
                                       rdfs:subPropertyOf fibo-sec-fund-civ:fundHasRelatedParty.
fibo-sec-fund-civ:hasPolicyTerms a owl:ObjectProperty;
                                 rdfs:domain fibo-sec-fund-civ:FundBondUnitCoupon;
                                 rdfs:isDefinedBy fibo-sec-fund-civ:;
                                 rdfs:label "has policy terms"@en;
                                 rdfs:range fibo-sec-fund-civ:FundCouponPolicy.
fibo-sec-fund-civ:hasPortfolio a owl:ObjectProperty;
                               rdfs:domain fibo-sec-sec-pls:CollectiveInvestmentVehicle;
                               rdfs:isDefinedBy fibo-sec-fund-civ:;
                               rdfs:label "has portfolio"@en;
                               rdfs:range fibo-sec-fund-civ:FundPortfolio.
fibo-sec-fund-civ:hasRelatedFundTerms a owl:ObjectProperty;
                                      rdfs:domain fibo-sec-sec-pls:CollectiveInvestmentVehicle;
                                      rdfs:isDefinedBy fibo-sec-fund-civ:;
                                      rdfs:label "has related fund terms"@en;
                                      rdfs:range fibo-sec-fund-civ:FundProcessingTerms;
                                      rdfs:subPropertyOf fibo-sec-fund-civ:hasRelatedTerms.
fibo-sec-fund-civ:hasRelatedTerms a owl:ObjectProperty;
                                  rdfs:isDefinedBy fibo-sec-fund-civ:;
                                  rdfs:label "has related terms"@en;
                                  rdfs:range fibo-fnd-agr-ctr:ContractualElement.
fibo-sec-fund-civ:hasSubscriptionTerms a owl:ObjectProperty;
                                       rdfs:domain fibo-sec-sec-pls:CollectiveInvestmentVehicle;
                                       rdfs:isDefinedBy fibo-sec-fund-civ:;
                                       rdfs:label "has subscription terms"@en;
                                       rdfs:range fibo-sec-fund-civ:FundSubscriptionTerms;
                                       rdfs:subPropertyOf fibo-sec-fund-civ:hasRelatedFundTerms.
fibo-sec-fund-civ:hasTradableUnit a owl:ObjectProperty;
                                  rdfs:domain fibo-sec-sec-pls:CollectiveInvestmentVehicle;
                                  rdfs:isDefinedBy fibo-sec-fund-civ:;
                                  rdfs:label "has tradable unit"@en;
                                  rdfs:range fibo-sec-fund-fund:FundUnit.
fibo-sec-fund-civ:hasTransferAgent a owl:ObjectProperty;
                                   rdfs:domain fibo-sec-sec-pls:CollectiveInvestmentVehicle;
                                   rdfs:isDefinedBy fibo-sec-fund-civ:;
                                   rdfs:label "has transfer agent"@en;
                                   rdfs:range fibo-sec-fund-civ:FundTransferAgent;
                                   rdfs:subPropertyOf fibo-sec-fund-civ:fundHasRelatedParty.
fibo-sec-fund-civ:historicPricingIndicator a owl:DatatypeProperty;
                                           rdfs:domain fibo-sec-fund-civ:NetAssetValueCalculationMethod;
                                           rdfs:isDefinedBy fibo-sec-fund-civ:;
                                           rdfs:label "historic pricing indicator"@en;
                                           rdfs:range xsd:boolean;
                                           skos:definition "Indicates whether the price is historic or forward."@en.
fibo-sec-fund-civ:holderMayReinvest a owl:DatatypeProperty;
                                    rdfs:domain fibo-sec-fund-civ:DistributingShareClass;
                                    rdfs:isDefinedBy fibo-sec-fund-civ:;
                                    rdfs:label "holder may reinvest"@en;
                                    rdfs:range xsd:boolean;
                                    skos:definition "Whether or not the holder may reinvest dividends in the fund."@en.
fibo-sec-fund-civ:holdingTransferable a owl:DatatypeProperty;
                                      rdfs:domain fibo-sec-fund-civ:FundProcessingGeneralTerms;
                                      rdfs:isDefinedBy fibo-sec-fund-civ:;
                                      rdfs:label "holding transferable"@en;
                                      rdfs:range xsd:boolean;
                                      skos:definition "Whether registered investors are able to transfer some or all of their holdings to third parties."@en.
fibo-sec-fund-civ:identifiesAssetTypesBy a owl:ObjectProperty;
                                         rdfs:domain fibo-sec-fund-civ:AssetClassStrategy;
                                         rdfs:isDefinedBy fibo-sec-fund-civ:;
                                         rdfs:label "identifies asset types by"@en;
                                         rdfs:range fibo-sec-sec-cls:FinancialInstrumentClassifier.
fibo-sec-fund-civ:implementsFundPolicy a owl:ObjectProperty;
                                       rdfs:domain fibo-sec-fund-civ:FundPortfolio;
                                       rdfs:isDefinedBy fibo-sec-fund-civ:;
                                       rdfs:label "implements fund policy"@en;
                                       rdfs:range fibo-sec-fund-civ:FundPortfolioInvestmentPolicy.
fibo-sec-fund-civ:inceptionDate a owl:ObjectProperty;
                                rdfs:domain fibo-sec-sec-pls:CollectiveInvestmentVehicle;
                                rdfs:isDefinedBy fibo-sec-fund-civ:;
                                rdfs:label "inception date"@en;
                                rdfs:range cmns-dt:Date;
                                skos:definition "Authorization date in the country of origin."@en.
fibo-sec-fund-civ:inceptionDate.1 a owl:ObjectProperty;
                                  rdfs:domain fibo-sec-fund-civ:FundShareClassUnit;
                                  rdfs:isDefinedBy fibo-sec-fund-civ:;
                                  rdfs:label "inception date"@en;
                                  rdfs:range cmns-dt:Date;
                                  skos:definition """Authorization date in the country of origin. Further Notes See definition in Inception Date for Fund. Separate fact exists here. Same definition used. EFAMA Review notes: Inception Date exists as soon as there is a prospectus, so it is a fact about a Share Class even if the share class is never formally issued or offered to the public. Legal structure exists even if something is not launched. Editor question: Review stated this was a fact about Share Class; confirm this fact does not apply to Bond and Note units, or was the term Share Class being used to mean all three? Meanwhile I have put the term \"Issue Date\" as a fact about all Fund Unit, as this is given a sa separate term in the EFAMA DD spreadsheet. MAy come clearer in the next version of that."""@en.
fibo-sec-fund-civ:includeRelatedFirms a owl:DatatypeProperty;
                                      rdfs:domain fibo-sec-fund-civ:OrganizationStrategy;
                                      rdfs:isDefinedBy fibo-sec-fund-civ:;
                                      rdfs:label "include related firms"@en;
                                      rdfs:range xsd:boolean;
                                      skos:definition "Whether or not the strategy includes firms which are related in some way to the referenced organization."@en.
fibo-sec-fund-civ:inclusion a owl:DatatypeProperty;
                            rdfs:domain fibo-sec-fund-civ:FundPortfolioInvestmentLimitations;
                            rdfs:isDefinedBy fibo-sec-fund-civ:;
                            rdfs:label "inclusion"@en;
                            rdfs:range xsd:boolean;
                            skos:definition "Whether the referred strategy is included. No means this description refers to the exclusion of what is described, from the portfolio."@en.
fibo-sec-fund-civ:initialApplicationForm a owl:ObjectProperty;
                                         rdfs:domain fibo-sec-fund-civ:FundSubscriptionTerms;
                                         rdfs:isDefinedBy fibo-sec-fund-civ:;
                                         rdfs:label "initial application form"@en;
                                         skos:definition "Physical application form for the initial subscription by the investor."@en.
fibo-sec-fund-civ:investmentFocus a owl:DatatypeProperty;
                                  rdfs:domain fibo-sec-fund-civ:PortfolioInvestmentStrategy;
                                  rdfs:isDefinedBy fibo-sec-fund-civ:;
                                  rdfs:label "investment focus"@en;
                                  rdfs:range xsd:string;
                                  skos:definition "The information about the area the fund is mostly invested into (for example stock market in Germany)."@en.
fibo-sec-fund-civ:isCalculatedIn a owl:ObjectProperty;
                                 rdfs:domain fibo-sec-fund-civ:NetAssetValueCalculationMethod;
                                 rdfs:isDefinedBy fibo-sec-fund-civ:;
                                 rdfs:label "is calculated in"@en;
                                 rdfs:range fibo-fnd-acc-cur:Currency.
fibo-sec-fund-civ:isUnitHolder a owl:ObjectProperty;
                               rdfs:domain fibo-be-oac-opty:Investor;
                               rdfs:isDefinedBy fibo-sec-fund-civ:;
                               rdfs:label "is unit holder"@en;
                               rdfs:range fibo-sec-fund-fund:FundUnit.
fibo-sec-fund-civ:issuePrice a owl:ObjectProperty;
                             rdfs:domain fibo-sec-fund-fund:FundUnit;
                             rdfs:isDefinedBy fibo-sec-fund-civ:;
                             rdfs:label "issue price"@en;
                             rdfs:range fibo-fnd-acc-cur:Price;
                             skos:definition "The price at which the Fund Unit was first issued."@en.
fibo-sec-fund-civ:launchDate a owl:DatatypeProperty;
                             rdfs:domain fibo-sec-sec-pls:CollectiveInvestmentVehicle;
                             rdfs:isDefinedBy fibo-sec-fund-civ:;
                             rdfs:label "launch date"@en;
                             skos:definition "Date of first NAV calculation and start of performance calculations"@en.
fibo-sec-fund-civ:limitedSharesAreIssued a owl:DatatypeProperty;
                                         rdfs:domain fibo-sec-fund-civ:FundShareClassUnit;
                                         rdfs:isDefinedBy fibo-sec-fund-civ:;
                                         rdfs:label "limited shares are issued"@en;
                                         rdfs:range xsd:boolean;
                                         skos:definition "Whether or not new shares can be issued in the fund. This is what makes it a closed end or open end fund."@en.
fibo-sec-fund-civ:mainFundOrderDesk a owl:DatatypeProperty;
                                    rdfs:domain fibo-sec-fund-civ:FundProcessingTerms;
                                    rdfs:isDefinedBy fibo-sec-fund-civ:;
                                    rdfs:label "main fund order desk"@en;
                                    rdfs:range xsd:boolean;
                                    skos:definition "Whether the fund order desk is the principal entity appointed by the fund to which orders should be submitted."@en.
fibo-sec-fund-civ:maximumDeviation a owl:ObjectProperty;
                                   rdfs:domain fibo-sec-fund-civ:PortfolioBenchmark;
                                   rdfs:isDefinedBy fibo-sec-fund-civ:;
                                   rdfs:label "maximum deviation"@en;
                                   rdfs:range cmns-qtu:Percentage;
                                   skos:definition "Maximum allowable deviation from the benchmark."@en.
fibo-sec-fund-civ:maximumInvestmentAmount a owl:ObjectProperty;
                                          rdfs:domain fibo-sec-fund-civ:FundPortfolioInvestmentLimitations;
                                          rdfs:isDefinedBy fibo-sec-fund-civ:;
                                          rdfs:label "maximum investment amount"@en;
                                          rdfs:range fibo-fnd-acc-cur:MonetaryAmount;
                                          skos:definition "Maximum amount that may be invested in the specified strategy."@en.
fibo-sec-fund-civ:maximumInvestmentPercentage a owl:ObjectProperty;
                                              rdfs:domain fibo-sec-fund-civ:FundPortfolioInvestmentLimitations;
                                              rdfs:isDefinedBy fibo-sec-fund-civ:;
                                              rdfs:label "maximum investment percentage"@en;
                                              rdfs:range cmns-qtu:Percentage;
                                              skos:definition "Maximum percentage that may be invested in the specified strategy."@en.
fibo-sec-fund-civ:maximumPurchasingFee a owl:ObjectProperty;
                                       rdfs:domain fibo-sec-fund-civ:FundSubscriptionTerms;
                                       rdfs:isDefinedBy fibo-sec-fund-civ:;
                                       rdfs:label "maximum purchasing fee"@en;
                                       rdfs:range fibo-fbc-pas-caa:Fee;
                                       skos:definition "Maximum percentage or fixed amount of money due when purchasing fund shares Definition origin:EFAMA DD"@en.
fibo-sec-fund-civ:maximumRedemptionAmount a owl:ObjectProperty;
                                          rdfs:domain fibo-sec-fund-civ:FundRedemptionTerms;
                                          rdfs:isDefinedBy fibo-sec-fund-civ:;
                                          rdfs:label "maximum redemption amount"@en;
                                          rdfs:range fibo-fnd-acc-cur:MonetaryAmount;
                                          skos:definition "Maximum quantity of securities, expressed as an amount that can be sold."@en.
fibo-sec-fund-civ:maximumRedemptionFee a owl:ObjectProperty;
                                       rdfs:domain fibo-sec-fund-civ:FundSubscriptionTerms;
                                       rdfs:isDefinedBy fibo-sec-fund-civ:;
                                       rdfs:label "maximum redemption fee"@en;
                                       rdfs:range fibo-fbc-pas-caa:Fee;
                                       skos:definition "Maximum percentage or fixed amount of money due when redeeming fund shares Definition origin:EFAMA DD"@en.
fibo-sec-fund-civ:maximumRedemptionPercentage a owl:ObjectProperty;
                                              rdfs:domain fibo-sec-fund-civ:FundRedemptionTerms;
                                              rdfs:isDefinedBy fibo-sec-fund-civ:;
                                              rdfs:label "maximum redemption percentage"@en;
                                              rdfs:range cmns-qtu:Percentage;
                                              skos:definition "Maximum quantity of securities, expressed as a percentage that can be sold."@en.
fibo-sec-fund-civ:maximumRedemptionUnits a owl:DatatypeProperty;
                                         rdfs:domain fibo-sec-fund-civ:FundRedemptionTerms;
                                         rdfs:isDefinedBy fibo-sec-fund-civ:;
                                         rdfs:label "maximum redemption units"@en;
                                         rdfs:range xsd:integer;
                                         skos:definition "Maximum number of shares/units that may be redeemed on a single dealing day."@en.
fibo-sec-fund-civ:mayAlsoBe a owl:ObjectProperty;
                            rdfs:domain fibo-sec-fund-fund:FundAdministrator;
                            rdfs:isDefinedBy fibo-sec-fund-civ:;
                            rdfs:label "may also be"@en;
                            rdfs:range fibo-sec-fund-civ:UnitIssuer;
                            skos:definition "The unit issuer would be the fund administrator (except when it is a Bond)."@en.
fibo-sec-fund-civ:minimumDeviation a owl:ObjectProperty;
                                   rdfs:domain fibo-sec-fund-civ:PortfolioBenchmark;
                                   rdfs:isDefinedBy fibo-sec-fund-civ:;
                                   rdfs:label "minimum deviation"@en;
                                   rdfs:range cmns-qtu:Percentage;
                                   skos:definition "Minimum allowable deviation from the benchmark."@en.
fibo-sec-fund-civ:minimumHoldingPeriod a owl:ObjectProperty;
                                       rdfs:domain fibo-sec-fund-civ:FundProcessingGeneralTerms;
                                       rdfs:isDefinedBy fibo-sec-fund-civ:;
                                       rdfs:label "minimum holding period"@en;
                                       rdfs:range cmns-dt:Duration;
                                       skos:definition "Period, in days, during which the units/shares must be held following their issue before redemption will be permitted."@en.
fibo-sec-fund-civ:minimumInitialSubscriptionAmount a owl:ObjectProperty;
                                                   rdfs:domain fibo-sec-fund-civ:FundSubscriptionTerms;
                                                   rdfs:isDefinedBy fibo-sec-fund-civ:;
                                                   rdfs:label "minimum initial subscription amount"@en;
                                                   rdfs:range fibo-fnd-acc-cur:MonetaryAmount;
                                                   skos:definition "Minimum initial subscription value."@en.
fibo-sec-fund-civ:minimumInitialSubscriptionUnits a owl:DatatypeProperty;
                                                  rdfs:domain fibo-sec-fund-civ:FundSubscriptionTerms;
                                                  rdfs:isDefinedBy fibo-sec-fund-civ:;
                                                  rdfs:label "minimum initial subscription units"@en;
                                                  rdfs:range xsd:integer;
                                                  skos:definition "Minimum initial number of units/shares that must be purchased."@en.
fibo-sec-fund-civ:minimumInvestmentAmount a owl:ObjectProperty;
                                          rdfs:domain fibo-sec-fund-civ:FundPortfolioInvestmentLimitations;
                                          rdfs:isDefinedBy fibo-sec-fund-civ:;
                                          rdfs:label "minimum investment amount"@en;
                                          rdfs:range fibo-fnd-acc-cur:MonetaryAmount;
                                          skos:definition "Minimum amount that has to be invested in the specified strategy."@en.
fibo-sec-fund-civ:minimumInvestmentPercentage a owl:ObjectProperty;
                                              rdfs:domain fibo-sec-fund-civ:FundPortfolioInvestmentLimitations;
                                              rdfs:isDefinedBy fibo-sec-fund-civ:;
                                              rdfs:label "minimum investment percentage"@en;
                                              rdfs:range cmns-qtu:Percentage;
                                              skos:definition "Minimum percentage that has to be invested in the specified strategy."@en.
fibo-sec-fund-civ:minimumRatingRestriction a owl:ObjectProperty;
                                           rdfs:domain fibo-sec-fund-civ:InvestmentRestriction;
                                           rdfs:isDefinedBy fibo-sec-fund-civ:;
                                           rdfs:label "minimum rating restriction"@en;
                                           rdfs:range fibo-fnd-arr-rt:RatingScore;
                                           skos:definition "The minimum rating of securities to be invested in."@en.
fibo-sec-fund-civ:minimumRemainingHoldingAmount a owl:ObjectProperty;
                                                rdfs:domain fibo-sec-fund-civ:FundProcessingGeneralTerms;
                                                rdfs:isDefinedBy fibo-sec-fund-civ:;
                                                rdfs:label "minimum remaining holding amount"@en;
                                                rdfs:range fibo-fnd-acc-cur:MonetaryAmount;
                                                skos:definition "Minimum value of units/shares that must be retained to avoid automatic redemption."@en.
fibo-sec-fund-civ:minimumRemainingHoldingUnits a owl:DatatypeProperty;
                                               rdfs:domain fibo-sec-fund-civ:FundProcessingGeneralTerms;
                                               rdfs:isDefinedBy fibo-sec-fund-civ:;
                                               rdfs:label "minimum remaining holding units"@en;
                                               rdfs:range xsd:integer;
                                               skos:definition "Minimum number of units/shares that must be retained to avoid automatic redemption."@en.
fibo-sec-fund-civ:minimumSubscriptionAmount a owl:ObjectProperty;
                                            rdfs:domain fibo-sec-fund-civ:FundSubscriptionTerms;
                                            rdfs:isDefinedBy fibo-sec-fund-civ:;
                                            rdfs:label "minimum subscription amount"@en;
                                            rdfs:range fibo-fnd-acc-cur:MonetaryAmount;
                                            skos:definition "Minimum subscription value for existing investors."@en.
fibo-sec-fund-civ:minimumSubscriptionUnits a owl:DatatypeProperty;
                                           rdfs:domain fibo-sec-fund-civ:FundSubscriptionTerms;
                                           rdfs:isDefinedBy fibo-sec-fund-civ:;
                                           rdfs:label "minimum subscription units"@en;
                                           rdfs:range xsd:integer;
                                           skos:definition "Minimum number of units/shares that must be purchased by existing investors."@en.
fibo-sec-fund-civ:name a owl:DatatypeProperty;
                       rdfs:domain fibo-sec-sec-pls:CollectiveInvestmentVehicle;
                       rdfs:isDefinedBy fibo-sec-fund-civ:;
                       rdfs:label "name"@en;
                       rdfs:range xsd:string;
                       skos:definition "Name of the investment fund."@en.
fibo-sec-fund-civ:name.1 a owl:DatatypeProperty;
                         rdfs:domain fibo-sec-fund-civ:FundPortfolioInvestmentPolicy;
                         rdfs:isDefinedBy fibo-sec-fund-civ:;
                         rdfs:label "name"@en;
                         rdfs:range xsd:string;
                         skos:definition "Name given to the defined strategy."@en.
fibo-sec-fund-civ:outlines a owl:ObjectProperty;
                           rdfs:domain fibo-sec-sec-iss:Prospectus;
                           rdfs:isDefinedBy fibo-sec-fund-civ:;
                           rdfs:label "outlines"@en;
                           rdfs:range fibo-sec-fund-civ:FundInvestmentObjective;
                           owl:inverseOf fibo-sec-fund-civ:statedIn.
fibo-sec-fund-civ:percentageInvested a owl:ObjectProperty;
                                     rdfs:domain fibo-sec-fund-civ:InvestmentRestriction;
                                     rdfs:isDefinedBy fibo-sec-fund-civ:;
                                     rdfs:label "percentage invested"@en;
                                     rdfs:range cmns-qtu:Percentage;
                                     skos:definition "The percentage of funds that is to be invested at any given time."@en.
fibo-sec-fund-civ:performanceFee a owl:ObjectProperty;
                                 rdfs:domain fibo-sec-fund-civ:FundSubscriptionTerms;
                                 rdfs:isDefinedBy fibo-sec-fund-civ:;
                                 rdfs:label "performance fee"@en;
                                 rdfs:range fibo-fbc-pas-caa:Fee;
                                 skos:definition "Fees paid for the achivements of predefined outperformance objectives Definition origin:EFAMA DD"@en.
fibo-sec-fund-civ:physicalDocumentRequired a owl:DatatypeProperty;
                                           rdfs:isDefinedBy fibo-sec-fund-civ:;
                                           rdfs:label "physical document required"@en;
                                           rdfs:range xsd:boolean;
                                           skos:definition "Whether a phsyical form is required through the main fund order desk. Yes: A phsyical form is required through the main fund order desk. No: A phsyical form is not required through the main fund order desk."@en.
fibo-sec-fund-civ:processingCountry a owl:ObjectProperty;
                                    rdfs:domain fibo-sec-fund-civ:FundProcessingTerms;
                                    rdfs:isDefinedBy fibo-sec-fund-civ:;
                                    rdfs:label "processing country"@en;
                                    rdfs:range cmns-loc:Country;
                                    skos:definition "Country in which the processing characteristic applies."@en.
fibo-sec-fund-civ:productGroupDescription a owl:DatatypeProperty;
                                          rdfs:domain fibo-sec-sec-pls:CollectiveInvestmentVehicle;
                                          rdfs:isDefinedBy fibo-sec-fund-civ:;
                                          rdfs:label "product group description"@en;
                                          rdfs:range xsd:string;
                                          skos:definition "Company specific description of a group of funds."@en.
fibo-sec-fund-civ:providesDepositaryServiceFor a owl:ObjectProperty;
                                               rdfs:domain fibo-sec-fund-civ:FundDepositary;
                                               rdfs:isDefinedBy fibo-sec-fund-civ:;
                                               rdfs:label "provides depositary service for"@en;
                                               rdfs:range fibo-sec-fund-fund:FundUnit.
fibo-sec-fund-civ:purchasingFee a owl:ObjectProperty;
                                rdfs:domain fibo-sec-fund-civ:FundSubscriptionTerms;
                                rdfs:isDefinedBy fibo-sec-fund-civ:;
                                rdfs:label "purchasing fee"@en;
                                rdfs:range fibo-fbc-pas-caa:Fee;
                                skos:definition "Actual percentage or fixed amount of money due when purchasing fund shares Definition origin:EFAMA DD"@en.
fibo-sec-fund-civ:redemptionCutoffDateTime a owl:ObjectProperty;
                                           rdfs:domain fibo-sec-fund-civ:FundRedemptionTerms;
                                           rdfs:isDefinedBy fibo-sec-fund-civ:;
                                           rdfs:label "redemption cutoff date time"@en;
                                           rdfs:range cmns-dt:DateTime;
                                           skos:definition "Last date/time at which an order to redeem can be given."@en.
fibo-sec-fund-civ:redemptionCycleInBusinessDays a owl:DatatypeProperty;
                                                rdfs:domain fibo-fbc-fi-stl:SettlementConvention;
                                                rdfs:isDefinedBy fibo-sec-fund-civ:;
                                                rdfs:label "redemption cycle in business days"@en;
                                                rdfs:range xsd:integer;
                                                skos:definition "The last business day following the day on which a redemption order is priced (T) by which settlement will be due for orders placed with the main Fund Order Desk. Alternatively, if proceeds will be paid following receipt of written renunciation, the last business day following receipt of the relevant renunciation documentation by the main Fund Order Desk (R) by which the proceeds will be sent."@en.
fibo-sec-fund-civ:redemptionDealingFrequency a owl:ObjectProperty;
                                             rdfs:domain fibo-sec-fund-civ:FundRedemptionTerms;
                                             rdfs:isDefinedBy fibo-sec-fund-civ:;
                                             rdfs:label "redemption dealing frequency"@en;
                                             rdfs:range fibo-fnd-dt-fd:RecurrenceInterval;
                                             skos:definition "Frequency at which the redemptions are done."@en.
fibo-sec-fund-civ:redemptionFee a owl:ObjectProperty;
                                rdfs:domain fibo-sec-fund-civ:FundSubscriptionTerms;
                                rdfs:isDefinedBy fibo-sec-fund-civ:;
                                rdfs:label "redemption fee"@en;
                                rdfs:range fibo-fbc-pas-caa:Fee;
                                skos:definition "Actual percentage or fixed amount of money due when redeeming fund shares Definition origin:EFAMA DD"@en.
fibo-sec-fund-civ:redemptionForm a owl:ObjectProperty;
                                 rdfs:domain fibo-sec-fund-civ:FundRedemptionTerms;
                                 rdfs:isDefinedBy fibo-sec-fund-civ:;
                                 rdfs:label "redemption form"@en;
                                 skos:definition "Physical written instruction/renunciation form for redemption of units/shares by the investor."@en.
fibo-sec-fund-civ:redemptionInAmountAllowed a owl:DatatypeProperty;
                                            rdfs:domain fibo-sec-fund-civ:FundRedemptionTerms;
                                            rdfs:isDefinedBy fibo-sec-fund-civ:;
                                            rdfs:label "redemption in amount allowed"@en;
                                            rdfs:range xsd:boolean;
                                            skos:definition "Whether redemptions in amount are allowed."@en.
fibo-sec-fund-civ:redemptionPeriod a owl:ObjectProperty;
                                   rdfs:domain fibo-sec-fund-civ:FundRedemptionTerms;
                                   rdfs:isDefinedBy fibo-sec-fund-civ:;
                                   rdfs:label "redemption period"@en;
                                   rdfs:range cmns-dt:DatePeriod;
                                   skos:definition "Specific period, eg, for some guaranteed funds, during which the units/shares may be redeemed."@en.
fibo-sec-fund-civ:registrationDate a owl:DatatypeProperty;
                                   rdfs:domain fibo-sec-sec-pls:CollectiveInvestmentVehicle;
                                   rdfs:isDefinedBy fibo-sec-fund-civ:;
                                   rdfs:label "registration date"@en;
                                   skos:definition "The date at which the fund is legally approved in a country other than the country of origin."@en.
fibo-sec-fund-civ:reinvestmentFrequency a owl:ObjectProperty;
                                        rdfs:domain fibo-sec-fund-civ:FundReinvestmentPolicy;
                                        rdfs:isDefinedBy fibo-sec-fund-civ:;
                                        rdfs:label "reinvestment frequency"@en;
                                        rdfs:range fibo-fnd-dt-fd:RecurrenceInterval;
                                        skos:definition "For units where there is Reinvestment distribution, the frequency with which the reinvestment takes place (this will be the same or less frequently than the Dividend Payment Frequency), otherwise this fact does not apply."@en.
fibo-sec-fund-civ:signatureRequired a owl:DatatypeProperty;
                                    rdfs:isDefinedBy fibo-sec-fund-civ:;
                                    rdfs:label "signature required"@en;
                                    rdfs:range xsd:boolean;
                                    skos:definition "Whether a phsyical form with the investor's written signature is required through the main fund order desk. Yes:A phsyical form with the investor's written signature is required through the main fund order desk."@en.
fibo-sec-fund-civ:statedDistributionFee a owl:ObjectProperty;
                                        rdfs:domain fibo-sec-sec-iss:Prospectus;
                                        rdfs:isDefinedBy fibo-sec-fund-civ:;
                                        rdfs:label "stated distribution fee"@en;
                                        rdfs:range fibo-fnd-acc-cur:MonetaryAmount.
fibo-sec-fund-civ:statedIn a owl:ObjectProperty;
                           rdfs:domain fibo-sec-fund-civ:FundInvestmentObjective;
                           rdfs:isDefinedBy fibo-sec-fund-civ:;
                           rdfs:label "stated in"@en;
                           rdfs:range fibo-sec-sec-iss:Prospectus.
fibo-sec-fund-civ:statedInvestmentAim a owl:DatatypeProperty;
                                      rdfs:domain fibo-sec-fund-civ:FundInvestmentObjective;
                                      rdfs:isDefinedBy fibo-sec-fund-civ:;
                                      rdfs:label "stated investment aim"@en;
                                      rdfs:range xsd:string;
                                      skos:definition "The stated aim of the Fund in words, e.g outperfom a given benchmark."@en.
fibo-sec-fund-civ:statedManagementFee a owl:ObjectProperty;
                                      rdfs:domain fibo-sec-sec-iss:Prospectus;
                                      rdfs:isDefinedBy fibo-sec-fund-civ:;
                                      rdfs:label "stated management fee"@en;
                                      rdfs:range fibo-fnd-acc-cur:MonetaryAmount;
                                      skos:definition "The fee that is stated in the Prospectus as being what is to be charged for management. Further notes: Can be monetary amount or a percentage or a combination. Action: simple type is wrong."@en.
fibo-sec-fund-civ:statedObjective a owl:DatatypeProperty;
                                  rdfs:domain fibo-sec-sec-iss:Prospectus;
                                  rdfs:isDefinedBy fibo-sec-fund-civ:;
                                  rdfs:label "stated objective"@en;
                                  rdfs:range xsd:string;
                                  skos:definition "The stated objective of the fund, in words."@en.
fibo-sec-fund-civ:stipulatesBenchmark a owl:ObjectProperty;
                                      rdfs:domain fibo-sec-fund-civ:FundInvestmentPolicy;
                                      rdfs:isDefinedBy fibo-sec-fund-civ:;
                                      rdfs:label "stipulates benchmark"@en;
                                      rdfs:range fibo-ind-ind-ind:MarketRate.
fibo-sec-fund-civ:subscriptionCutoffDateTime a owl:ObjectProperty;
                                             rdfs:domain fibo-sec-fund-civ:FundSubscriptionTerms;
                                             rdfs:isDefinedBy fibo-sec-fund-civ:;
                                             rdfs:label "subscription cutoff date time"@en;
                                             rdfs:range cmns-dt:DateTime;
                                             skos:definition "Last date/time at which an order to subscribe can be given."@en.
fibo-sec-fund-civ:subscriptionDealingFrequency a owl:ObjectProperty;
                                               rdfs:domain fibo-sec-fund-civ:FundSubscriptionTerms;
                                               rdfs:isDefinedBy fibo-sec-fund-civ:;
                                               rdfs:label "subscription dealing frequency"@en;
                                               rdfs:range fibo-fnd-dt-fd:RecurrenceInterval;
                                               skos:definition "Frequency at which the subscriptions are done."@en.
fibo-sec-fund-civ:subscriptionPeriod a owl:ObjectProperty;
                                     rdfs:domain fibo-sec-fund-civ:FundSubscriptionTerms;
                                     rdfs:isDefinedBy fibo-sec-fund-civ:;
                                     rdfs:label "subscription period"@en;
                                     rdfs:range cmns-dt:DatePeriod;
                                     skos:definition "Specific period, eg, for some guaranteed funds, during which the units/shares may be subscribed to."@en.
fibo-sec-fund-civ:subscriptionsInAmountAllowed a owl:DatatypeProperty;
                                               rdfs:domain fibo-sec-fund-civ:FundSubscriptionTerms;
                                               rdfs:isDefinedBy fibo-sec-fund-civ:;
                                               rdfs:label "subscriptions in amount allowed"@en;
                                               rdfs:range xsd:boolean;
                                               skos:definition "Whether subscriptions in amount are allowed."@en.
fibo-sec-fund-civ:subsequentApplicationForm a owl:ObjectProperty;
                                            rdfs:domain fibo-sec-fund-civ:FundSubscriptionTerms;
                                            rdfs:isDefinedBy fibo-sec-fund-civ:;
                                            rdfs:label "subsequent application form"@en;
                                            skos:definition "Physical application form for subsequent investments by the same investor."@en.
fibo-sec-fund-civ:supervisedBy a owl:ObjectProperty;
                               rdfs:domain fibo-sec-sec-pls:CollectiveInvestmentVehicle;
                               rdfs:isDefinedBy fibo-sec-fund-civ:;
                               rdfs:label "supervised by"@en;
                               rdfs:range fibo-sec-fund-civ:FundSupervisoryAuthority.
fibo-sec-fund-civ:switchingChargeable a owl:DatatypeProperty;
                                      rdfs:domain fibo-sec-fund-civ:FundProcessingGeneralTerms;
                                      rdfs:isDefinedBy fibo-sec-fund-civ:;
                                      rdfs:label "switching chargeable"@en;
                                      rdfs:range xsd:boolean;
                                      skos:definition "Whether a switching charge for changing between sub-funds of the same umbrella can be applied."@en.
fibo-sec-fund-civ:switchingFee a owl:ObjectProperty;
                               rdfs:domain fibo-sec-fund-civ:FundSubscriptionTerms;
                               rdfs:isDefinedBy fibo-sec-fund-civ:;
                               rdfs:label "switching fee"@en;
                               rdfs:range fibo-fbc-pas-caa:Fee;
                               skos:definition "Actual percentage or fixed amount of money due when switching to another fund. Definition origin:EFAMA DD"@en.
fibo-sec-fund-civ:trackingError a owl:ObjectProperty;
                                rdfs:domain fibo-sec-fund-civ:InvestmentRestriction;
                                rdfs:isDefinedBy fibo-sec-fund-civ:;
                                rdfs:label "tracking error"@en;
                                rdfs:range cmns-qtu:Percentage;
                                skos:definition "See RiskFactors narrative in EFAMA DD"@en.
fibo-sec-fund-civ:typeOfSecurities a owl:DatatypeProperty;
                                   rdfs:domain fibo-sec-fund-civ:InvestmentRestriction;
                                   rdfs:isDefinedBy fibo-sec-fund-civ:;
                                   rdfs:label "type of securities"@en;
                                   rdfs:range xsd:string;
                                   skos:definition "The type of securities or other holdings that may be invested in."@en.
fibo-sec-fund-civ:valuationFrequency a owl:ObjectProperty;
                                     rdfs:domain fibo-sec-fund-civ:NetAssetValueCalculationMethod;
                                     rdfs:isDefinedBy fibo-sec-fund-civ:;
                                     rdfs:label "valuation frequency"@en;
                                     rdfs:range fibo-fnd-dt-fd:RecurrenceInterval;
                                     skos:definition "Frequency of the net asset value calculation."@en.
fibo-sec-fund-civ:valuationFrequencyTextualDescription a owl:DatatypeProperty;
                                                       rdfs:domain fibo-sec-fund-civ:NetAssetValueCalculationMethod;
                                                       rdfs:isDefinedBy fibo-sec-fund-civ:;
                                                       rdfs:label "valuation frequency textual description"@en;
                                                       rdfs:range xsd:string;
                                                       skos:definition "Description of the frequency of the net asset value calculation."@en.
fibo-sec-fund-civ:valueAtRisk a owl:ObjectProperty;
                              rdfs:domain fibo-sec-fund-civ:InvestmentRestriction;
                              rdfs:isDefinedBy fibo-sec-fund-civ:;
                              rdfs:label "value at risk"@en;
                              rdfs:range cmns-qtu:Percentage;
                              skos:definition "See RiskClassification_NameOf in EFAMA DD Applies to Fund not Portfolio."@en.
fibo-sec-fund-fund:FundContract a owl:Class;
                                rdfs:subClassOf [a owl:Restriction ; 
                                                 owl:onProperty fibo-fnd-agr-ctr:isEvidencedBy ; 
                                                 owl:someValuesFrom fibo-sec-fund-civ:FundLegalFormDocumentation];
                                cmns-av:explanatoryNote """From ISO FIBIM \"Umbrella Fund\" narrative: In securities, a collective investment scheme that has a contractual or a corporate form. When it has a contractual form, a fund is constituted under either the law of contract or under the trust law and thus it is not a legal entity. In its corporate form, a fund is a legal entity and is structured as a company."""@en.
fibo-sec-fund-fund:FundUnit a owl:Class;
                            rdfs:subClassOf [a owl:Restriction ; 
                                             owl:onProperty fibo-sec-fund-civ:hasDetails ; 
                                             owl:someValuesFrom fibo-sec-fund-civ:NetAssetValueCalculationMethod],
                                            [a owl:Restriction ; 
                                             owl:onProperty fibo-sec-fund-civ:hasFundProcessingTerms ; 
                                             owl:someValuesFrom fibo-sec-fund-civ:FundProcessingGeneralTerms],
                                            [a owl:Restriction ; 
                                             owl:onProperty fibo-sec-fund-civ:hasFundProcessingTerms ; 
                                             owl:someValuesFrom fibo-sec-fund-civ:FundRedemptionTerms];
                            cmns-av:explanatoryNote "If it is a closed fund, you can still trade the units. You trade back with the fund. Not with a counterparty. Therefore this is a tradable contract, though it may not necessarily be a transferable contract."@en.
fibo-sec-sec-pls:CollectiveInvestmentVehicle a owl:Class;
                                             rdfs:subClassOf [a owl:Restriction ; 
                                                              owl:onProperty fibo-fbc-fi-fi:isLegallyRecordedIn ; 
                                                              owl:someValuesFrom cmns-rga:Jurisdiction],
                                                             [a owl:Restriction ; 
                                                              owl:onProperty fibo-fnd-acc-cur:hasCurrency ; 
                                                              owl:someValuesFrom fibo-fnd-acc-cur:Currency],
                                                             [a owl:Restriction ; 
                                                              owl:onProperty fibo-fnd-gao-obj:hasStrategy ; 
                                                              owl:someValuesFrom fibo-sec-fund-civ:FundUnitDistributionMethod],
                                                             [a owl:Restriction ; 
                                                              owl:onProperty fibo-fnd-rel-rel:isIssuedBy ; 
                                                              owl:someValuesFrom fibo-sec-fund-civ:UnitIssuer],
                                                             [a owl:Restriction ; 
                                                              owl:onProperty fibo-sec-fund-civ:administeredBy ; 
                                                              owl:someValuesFrom fibo-sec-fund-fund:FundAdministrator],
                                                             [a owl:Restriction ; 
                                                              owl:onProperty fibo-sec-fund-civ:advisedBy ; 
                                                              owl:someValuesFrom fibo-fbc-fct-fse:RegisteredInvestmentAdvisor],
                                                             [a owl:Restriction ; 
                                                              owl:onProperty fibo-sec-fund-civ:distributedBy ; 
                                                              owl:someValuesFrom fibo-sec-fund-civ:FundDistributor],
                                                             [a owl:Restriction ; 
                                                              owl:onProperty fibo-sec-fund-civ:fundHasRelatedParty ; 
                                                              owl:someValuesFrom fibo-sec-fund-civ:FundsProcessingParty],
                                                             [a owl:Restriction ; 
                                                              owl:onProperty fibo-sec-fund-civ:hasAdditionalInformation ; 
                                                              owl:someValuesFrom fibo-sec-fund-civ:OtherInvestmentFundInformation],
                                                             [a owl:Restriction ; 
                                                              owl:onProperty fibo-sec-fund-civ:hasAuditor ; 
                                                              owl:someValuesFrom fibo-be-oac-exec:ExternalAuditor],
                                                             [a owl:Restriction ; 
                                                              owl:onProperty fibo-sec-fund-civ:hasDataProvider ; 
                                                              owl:someValuesFrom fibo-be-fct-pub:MarketDataProvider],
                                                             [a owl:Restriction ; 
                                                              owl:onProperty fibo-sec-fund-civ:hasDepository ; 
                                                              owl:someValuesFrom fibo-sec-fund-civ:FundDepositary],
                                                             [a owl:Restriction ; 
                                                              owl:onProperty fibo-sec-fund-civ:hasFundPolicy ; 
                                                              owl:someValuesFrom fibo-sec-fund-civ:FundInvestmentPolicy],
                                                             [a owl:Restriction ; 
                                                              owl:onProperty fibo-sec-fund-civ:hasManagementCompany ; 
                                                              owl:someValuesFrom fibo-sec-fund-fund:FundManager],
                                                             [a owl:Restriction ; 
                                                              owl:onProperty fibo-sec-fund-civ:hasRelatedFundTerms ; 
                                                              owl:someValuesFrom fibo-sec-fund-civ:FundProcessingTerms],
                                                             [a owl:Restriction ; 
                                                              owl:onProperty fibo-sec-fund-civ:hasSubscriptionTerms ; 
                                                              owl:someValuesFrom fibo-sec-fund-civ:FundSubscriptionTerms],
                                                             [a owl:Restriction ; 
                                                              owl:onProperty fibo-sec-fund-civ:hasTransferAgent ; 
                                                              owl:someValuesFrom fibo-sec-fund-civ:FundTransferAgent],
                                                             [a owl:Restriction ; 
                                                              owl:onProperty fibo-sec-fund-civ:supervisedBy ; 
                                                              owl:someValuesFrom fibo-sec-fund-civ:FundSupervisoryAuthority],
                                                             [a owl:Restriction ; 
                                                              owl:onProperty cmns-dsg:isDescribedBy ; 
                                                              owl:someValuesFrom fibo-sec-sec-iss:Prospectus];
                                             cmns-av:explanatoryNote "From EFAMA DD: The word fund can refer to either an investment pool, umbrella or share class, and is commonly refered to as a collective investment vehicle (can have ISIN or not). The meaning here is for the investment pool (of which an Umbrella fund is also one such) and not to the share class."@en.
fibo-sec-sec-iss:Prospectus a owl:Class;
                            rdfs:subClassOf [a owl:Restriction ; 
                                             owl:onProperty fibo-sec-fund-civ:outlines ; 
                                             owl:someValuesFrom fibo-sec-fund-civ:FundInvestmentObjective];
                            skos:editorialNote "EFAMA Review description for this: The fund is issued with a prospectus; there is material in the prospectus that is binding; material that is expected but not binding, and information that may or may not be in the prospectus or a given fund."@en;
                            cmns-av:explanatoryNote "This document includes facts about the fund investment objective, investment focus and other details of the fund. Some of this information becomes binding on the fund once it is issued, while other information is guidelines only.".
